Rewrite call datatypes, semantics and implementation

pancake/proofs/pan_to_crepProofScript.sml
@@ -159,9 +159,20 @@ Definition ooHD_def:
   (ooHD (n::ns) = n)
 End
 
-Definition uassigned_eid_def:
-  uassigned_eid (emap:panLang$eid  |-> shape # num) =
-  MAX_SET (IMAGE SND (FRANGE emap)) + 1
+
+Definition assign_ret_def:
+  assign_ret ns =
+    nested_seq (MAP2 Assign ns (load_globals 0w (LENGTH ns)))
+End
+
+
+Definition declared_handler_def:
+  declared_handler sh mv =
+    if size_of_shape sh = 0 then Dec mv (Const 0w)
+    else
+      let nvars = GENLIST (λx. mv + SUC x) (size_of_shape sh);
+          vs = load_globals 0w (LENGTH nvars) in
+      nested_decs nvars vs
 End
 
 
@@ -227,7 +238,7 @@ Definition compile_prog_def:
       let temps = GENLIST (λx. ctxt.max_var + SUC x) (size_of_shape sh) in
       if size_of_shape sh = LENGTH (e::es)
       then Seq (nested_decs temps (e::es)
-                (nested_seq (store_globals 0w (MAP Var temps)))) (Raise n (Const 0w))
+                (nested_seq (store_globals 0w (MAP Var temps)))) (Raise n e)
       else Skip)
     | NONE => Skip) /\
   (compile_prog ctxt (Seq p p') =
@@ -250,6 +261,72 @@ Definition compile_prog_def:
        args = FLAT (MAP FST cexps) in
     case cs of
     | ce::ces =>
+     (case rtyp of
+       | Tail => Call Tail ce args
+       | Ret rt hdl =>
+         (case FLOOKUP ctxt.var_nums rt of
+          | SOME (One, n::ns) =>
+            (case hdl of
+              | NONE => Call (Ret n Skip NONE) ce args
+              | SOME (Handle eid evar p) =>
+                (case FLOOKUP ctxt.eid_map eid of
+                  | NONE => Call (Ret n Skip NONE) ce args
+                  | SOME (sh,neid) =>
+                    let vmax = ctxt.max_var;
+                        nvars = if size_of_shape sh = 0 then [vmax + 1]
+                                else GENLIST (λx. vmax + SUC x) (size_of_shape sh);
+                        nvmax = if size_of_shape sh = 0 then (vmax + 1) else (vmax + size_of_shape sh);
+                        nctxt = ctxt with <|var_nums := ctxt.var_nums |+ (evar, (sh, nvars));
+                                            max_var := nvmax|>;
+                        hndl_prog = declared_handler sh vmax (compile_prog nctxt p) in
+                    Call (Ret n Skip (SOME (Handle neid hndl_prog))) ce args))
+          | SOME (Comb sh, ns) =>
+            (case hdl of
+              | NONE => Call (Ret (if size_of_shape (Comb sh) = 1 then (ooHD ns) else (ctxt.max_var + 1))
+                                  (if 1 <= size_of_shape (Comb sh) then Skip else (assign_ret ns)) NONE) ce args
+              | SOME (Handle eid evar p) =>
+                (case FLOOKUP ctxt.eid_map eid of
+                  | NONE => Call (Ret (if size_of_shape (Comb sh) = 1 then (ooHD ns) else (ctxt.max_var + 1))
+                                      (if 1 <= size_of_shape (Comb sh) then Skip else (assign_ret ns)) NONE) ce args
+                  | SOME (esh,neid) =>
+                    let vmax = ctxt.max_var;
+                        nvars = if size_of_shape esh = 0 then [vmax + 1]
+                                else GENLIST (λx. vmax + SUC x) (size_of_shape esh);
+                        nvmax = if size_of_shape esh = 0 then (vmax + 1) else (vmax + size_of_shape esh);
+                        nctxt = ctxt with <|var_nums := ctxt.var_nums |+ (evar, (esh, nvars));
+                                            max_var := nvmax|>;
+                        hndl_prog = declared_handler esh vmax (compile_prog nctxt p) in
+                    Call (Ret (if size_of_shape (Comb sh) = 1 then (ooHD ns) else (vmax + 2))
+                              (if 1 <= size_of_shape (Comb sh) then Skip else (assign_ret ns))
+                              (SOME (Handle neid hndl_prog))) ce args))
+          | _ =>
+             (case hdl of
+              | NONE => Call Tail ce args
+              | SOME (Handle eid evar p) =>
+                (case FLOOKUP ctxt.eid_map eid of
+                   | NONE => Call Tail ce args
+                   | SOME (sh,neid) =>
+                     let vmax = ctxt.max_var;
+                         nvars = if size_of_shape sh = 0 then [vmax + 1]
+                                 else GENLIST (λx. vmax + SUC x) (size_of_shape sh);
+                         nvmax = if size_of_shape sh = 0 then (vmax + 1) else (vmax + size_of_shape sh);
+                         nctxt = ctxt with <|var_nums := ctxt.var_nums |+ (evar, (sh, nvars));
+                                             max_var := nvmax|>;
+                         hndl_prog = declared_handler sh vmax (compile_prog nctxt p) in
+                     Call (Ret (vmax + 2) Skip (SOME (Handle neid hndl_prog))) ce args))))
+    | [] => Skip) /\
+  (compile_prog ctxt (ExtCall f v1 v2 v3 v4) = ARB) /\
+  (compile_prog ctxt Tick = Tick)
+End
+
+
+(*
+  (compile_prog ctxt (Call rtyp e es) =
+   let (cs, sh) = compile_exp ctxt e;
+       cexps = MAP (compile_exp ctxt) es;
+       args = FLAT (MAP FST cexps) in
+    case cs of
+    | ce::ces =>
        (case rtyp of
        | Tail => Call Tail ce args
        | Ret rt =>
@@ -261,6 +338,8 @@ Definition compile_prog_def:
             else nested_seq (Call (Ret (ctxt.max_var + 1)) ce args ::
                                              MAP2 Assign ns (load_globals 0w (LENGTH ns)))
          | NONE =>  Call Tail ce args)
+
+
        | Handle rt eid evar p =>
           (case FLOOKUP ctxt.eid_map eid of
            | SOME (One,neid) =>
@@ -268,69 +347,53 @@ Definition compile_prog_def:
                | SOME (One, en::ens) =>
                   (case FLOOKUP ctxt.var_nums rt of
                     | SOME (One, n::ns) => Call (Handle n neid en (compile_prog ctxt p)) ce args
-                    | SOME (One, []) => Call Tail ce args
+                    | SOME (One, []) => Call (Handle (ctxt.max_var + 1) neid en (compile_prog ctxt p)) ce args
                     | SOME (Comb sh, ns) =>
                        if size_of_shape (Comb sh) = 1 then Call (Handle (ooHD ns) neid en (compile_prog ctxt p)) ce args
-                       else nested_seq (Call (Handle (ctxt.max_var + 1) neid en (compile_prog ctxt p)) ce args ::
-                                        MAP2 Assign ns (load_globals 0w (LENGTH ns)))
-                    | NONE =>  Call Tail ce args)
+                       else Seq (AppCode ce (assign_ret ns))
+                                (Call (Handle (ctxt.max_var + 1) neid en (compile_prog ctxt p)) ce args)
+                    | NONE =>  Call (Handle (ctxt.max_var + 1) neid en (compile_prog ctxt p)) ce args)
                | _ =>
                (case FLOOKUP ctxt.var_nums rt of
-                | SOME (One, n::ns) => Call (Handle n (uassigned_eid ctxt.eid_map) (ctxt.max_var + 1) (compile_prog ctxt p)) ce args
+                | SOME (One, n::ns) => Call (Ret n) ce args
                 | SOME (One, []) => Call Tail ce args
                 | SOME (Comb sh, ns) =>
-                if size_of_shape (Comb sh) = 1 then Call (Handle (ooHD ns) (uassigned_eid ctxt.eid_map)
-                                                          (ctxt.max_var + 1) (compile_prog ctxt p)) ce args
-                else nested_seq (Call (Handle (ctxt.max_var + 1) (uassigned_eid ctxt.eid_map)
-                                       (ctxt.max_var + 2) (compile_prog ctxt p)) ce args ::
+                if size_of_shape (Comb sh) = 1 then Call (Ret (ooHD ns)) ce args
+                else nested_seq (Call (Ret (ctxt.max_var + 1)) ce args ::
                                   MAP2 Assign ns (load_globals 0w (LENGTH ns)))
                 | NONE =>  Call Tail ce args))
            | SOME (Comb sh, n) => Call Tail ce args (* Remaining *)
            | NONE =>
              (case FLOOKUP ctxt.var_nums rt of
-              | SOME (One, n::ns) => Call (Handle n (uassigned_eid ctxt.eid_map) (ctxt.max_var + 1) (compile_prog ctxt p)) ce args
+              | SOME (One, n::ns) => Call (Ret n) ce args
               | SOME (One, []) => Call Tail ce args
               | SOME (Comb sh, ns) =>
-                 if size_of_shape (Comb sh) = 1 then Call (Handle (ooHD ns) (uassigned_eid ctxt.eid_map)
-                                                           (ctxt.max_var + 1) (compile_prog ctxt p)) ce args
-                 else nested_seq (Call (Handle (ctxt.max_var + 1) (uassigned_eid ctxt.eid_map)
-                                        (ctxt.max_var + 2) (compile_prog ctxt p)) ce args ::
-                                   MAP2 Assign ns (load_globals 0w (LENGTH ns)))
-              | NONE =>  Call Tail ce args)))
+                if size_of_shape (Comb sh) = 1 then Call (Ret (ooHD ns)) ce args
+                else nested_seq (Call (Ret (ctxt.max_var + 1)) ce args ::
+                                  MAP2 Assign ns (load_globals 0w (LENGTH ns)))
+         | NONE =>  Call Tail ce args)))
     | [] => Skip) /\
-  (compile_prog ctxt (ExtCall f v1 v2 v3 v4) = ARB) /\
-  (compile_prog ctxt Tick = Tick)
-End
+
+*)
+
 
 (* state relation *)
 
 val s = ``(s:('a,'ffi) panSem$state)``
 
-
 Definition excp_rel_def:
   excp_rel ctxt seids teids <=>
   FDOM seids =  FDOM ctxt.eid_map /\
-  (!e e' sh sh' n n'.
-    FLOOKUP ctxt.eid_map e = SOME (sh,n) /\
-    FLOOKUP ctxt.eid_map e' = SOME (sh',n') /\
-    n = n' ==> e = e') /\
-  (IMAGE SND (FRANGE ctxt.eid_map) = set teids)
-End
-
-
-(*
-Definition excp_rel_def:
-  excp_rel ctxt seids teids <=>
   (∀e sh.
   FLOOKUP seids e = SOME sh ==>
-  ?n. FLOOKUP ctxt.eid_map e = SOME (sh,n)) /\
+  (?n. FLOOKUP ctxt.eid_map e = SOME (sh,n))) /\
   (!e e' sh sh' n n'.
     FLOOKUP ctxt.eid_map e = SOME (sh,n) /\
     FLOOKUP ctxt.eid_map e' = SOME (sh',n') /\
     n = n' ==> e = e') /\
   (IMAGE SND (FRANGE ctxt.eid_map) = set teids)
 End
-*)
+
 
 Definition ctxt_max_def:
   ctxt_max (n:num) fm <=>
@@ -3073,6 +3136,13 @@ Proof
   cheat
 QED
 
+Theorem fdom_eq_flookup_none:
+  FDOM f = FDOM g /\ FLOOKUP f x = NONE ==>
+    FLOOKUP g x = NONE
+Proof
+  cheat
+QED
+
 Theorem compile_Raise:
   ^(get_goal "compile_prog _ (panLang$Raise _ _)")
 Proof
@@ -3085,10 +3155,7 @@ Proof
   disch_then drule_all >>
   strip_tac >> rveq >> rfs [] >>
   TOP_CASE_TAC
-  >- (fs [excp_rel_def] >> drule fdom_eq_flookup_some >>
-      disch_then drule >> fs []) >>
-
-
+  >- (fs [excp_rel_def] >> first_x_assum drule_all >> fs []) >>
   TOP_CASE_TAC >> fs [] >> rveq >>
   TOP_CASE_TAC >> fs [] >> rveq
   >- (
@@ -4036,6 +4103,75 @@ Proof
   cases_on ‘ys’ >> fs []
 QED
 
+
+Theorem max_set_list_max:
+  !xs. MAX_SET (set xs) = list_max xs
+Proof
+  Induct >> rw [] >> fs [list_max_def] >>
+  ‘FINITE (set xs)’ by fs [] >>
+  drule (MAX_SET_THM |> CONJUNCT2) >>
+  disch_then (qspec_then ‘h’ assume_tac) >>
+  fs [] >>
+  TOP_CASE_TAC >>fs [MAX_DEF]
+QED
+
+Theorem list_max_add_not_mem:
+  !xs. ~MEM (list_max xs + 1) xs
+Proof
+  Induct >> rw [] >> fs [list_max_def] >>
+  CCONTR_TAC >> fs [] >>
+  every_case_tac >> fs [list_max_def] >>
+  ntac 2 (pop_assum mp_tac) >> pop_assum kall_tac >>
+  qid_spec_tac ‘xs’ >>
+  Induct >> rw [] >> fs [list_max_def]
+QED
+
+Theorem set_eq_membership:
+  a = b ∧ x ∈ a ==> x ∈ b
+Proof
+  rw [] >> fs[]
+QED
+
+
+Theorem evaluate_append_code_intro:
+  eval s e = SOME (Label f) /\
+  FLOOKUP s.code f =  SOME (vs, prog) ==>
+  evaluate (Seq (AppCode e p) q,s) = evaluate (q, s with code := s.code |+ (f, (vs,Seq prog p)))
+Proof
+  rw [] >>
+  fs [evaluate_def]
+QED
+
+Theorem eval_upde_code_eq:
+  !s e v f ns p.
+  crepSem$eval s e = SOME v /\
+  FLOOKUP s.code f  <> NONE  ==>
+  eval (s with code := s.code |+ (f,ns,p)) e = SOME v
+Proof
+  ho_match_mp_tac eval_ind >>
+  rpt conj_tac >> rpt gen_tac >> strip_tac >>
+  TRY (fs [eval_def] >> every_case_tac >>
+       fs [FLOOKUP_UPDATE, mem_load_def] >>
+       rveq >> fs [] >>
+       every_case_tac >> fs [] >> NO_TAC) >>
+  rw [] >>
+  fs [eval_def] >> every_case_tac >> fs [] >>
+  rveq >> fs [] >> cheat
+QED
+
+Theorem opt_mmap_eval_upde_code_eq:
+  !s es vs f ns p.
+  OPT_MMAP (crepSem$eval s) es = SOME vs /\
+  FLOOKUP s.code f  <> NONE  ==>
+   OPT_MMAP (eval (s with code := s.code |+ (f,ns,p))) es = SOME vs
+Proof
+  rw [] >>
+  fs [opt_mmap_eq_some, MAP_EQ_EVERY2] >>
+  fs [LIST_REL_EL_EQN] >> rw [] >>
+  ho_match_mp_tac eval_upde_code_eq >> fs []
+QED
+
+
 Theorem ctxt_fc_code_vars_eq:
     (ctxt_fc cvs em vs shs ns).code_vars = cvs
 Proof
@@ -4165,7 +4301,6 @@ Proof
   fs [EVERY2_MAP]
 QED
 
-
 val clock_zero_tail_rt_tac =
     fs [evaluate_def] >>
     TOP_CASE_TAC >> fs [] >>
@@ -4213,8 +4348,41 @@ val clock_zero_nested_seq_rt_tac =
 val rels_empty_tac =
     fs [Abbr ‘nctxt’, state_rel_def, ctxt_fc_code_vars_eq, ctxt_fc_eid_map_eq,
         excp_rel_def, empty_locals_def, panSemTheory.empty_locals_def, code_rel_def,
-        globals_lookup_def] >>
-    rw [] >> first_x_assum drule_all >> fs []
+        globals_lookup_def]
+
+val clock_zero_append_code_tac =
+     qpat_x_assum ‘SOME (Label fname) = eval t x0’ (assume_tac o GSYM) >>
+     qmatch_goalsub_abbrev_tac ‘evaluate (Seq (AppCode x0 ar) pc, _)’ >>
+     drule evaluate_append_code_intro >>
+     fs [panSemTheory.lookup_code_def, CaseEq "option", CaseEq "prod"] >> rveq >>
+     drule code_rel_imp >>
+     disch_then drule >>
+     strip_tac >> fs [] >>
+     fs [lookup_code_def] >>
+     drule (INST_TYPE [``:'c``|->``:num``] list_rel_length_shape_of_flatten) >>
+     disch_then (qspec_then ‘ns’ mp_tac) >>
+     fs [] >> strip_tac >>
+     disch_then (qspecl_then [‘pc’, ‘ar’] assume_tac) >>
+     fs [] >> pop_assum kall_tac >>
+     qmatch_goalsub_abbrev_tac ‘evaluate (_, tnew)’ >>
+     fs [Abbr ‘pc’, evaluate_def] >>
+     ‘eval tnew x0 = eval t x0’ by (
+       fs [Abbr ‘tnew’] >>
+       match_mp_tac eval_upde_code_eq >> fs []) >>
+     fs [] >>
+     ‘OPT_MMAP (eval t)
+      (FLAT (MAP FST (MAP (compile_exp ctxt) argexps))) = SOME (FLAT (MAP flatten args))’ by (
+       fs [opt_mmap_eq_some] >> metis_tac [eval_map_comp_exp_flat_eq]) >>
+     qmatch_asmsub_abbrev_tac ‘t.code |+ (fname,ns,nc)’ >>
+     drule opt_mmap_eval_upde_code_eq >>
+     disch_then (qspecl_then [‘fname’, ‘ns’, ‘nc’] assume_tac) >>
+     fs [Abbr ‘tnew’, lookup_code_def, FLOOKUP_UPDATE] >>
+     drule (INST_TYPE [``:'c``|->``:num``] list_rel_length_shape_of_flatten) >>
+     disch_then (qspec_then ‘ns’ mp_tac) >>
+     fs [FLOOKUP_UPDATE] >>
+     ‘t.clock = 0’ by fs [state_rel_def] >> fs [] >>
+     fs [state_rel_def, empty_locals_def, panSemTheory.empty_locals_def] >>
+     cheat (* need to update code_rel *)
 
 
 val call_tail_ret_impl_tac =
@@ -4243,8 +4411,7 @@ val call_tail_ret_impl_tac =
       fs []) >>
      strip_tac >> fs [] >>
      fs [state_rel_def, Abbr ‘nctxt’, code_rel_def, ctxt_fc_code_vars_eq,
-         panSemTheory.empty_locals_def, empty_locals_def, ctxt_fc_eid_map_eq, excp_rel_def] >>
-     rw [] >> first_x_assum drule_all >> fs []
+         panSemTheory.empty_locals_def, empty_locals_def, ctxt_fc_eid_map_eq, excp_rel_def]
 
 
 val call_nested_seq_ret_impl_tac =
@@ -4276,8 +4443,8 @@ val call_nested_seq_ret_impl_tac =
     strip_tac >> fs [] >>
     rveq >> fs [] >>
     fs [Abbr ‘nctxt’, state_rel_def, ctxt_fc_code_vars_eq, ctxt_fc_eid_map_eq,
-        empty_locals_def, panSemTheory.empty_locals_def, code_rel_def, ctxt_fc_eid_map_eq, excp_rel_def] >>
-     rw [] >> first_x_assum drule_all >> fs []
+        empty_locals_def, panSemTheory.empty_locals_def, code_rel_def, ctxt_fc_eid_map_eq, excp_rel_def]
+
 
 val eval_call_impl_only_tac =
      fs [evaluate_def] >>
@@ -4332,7 +4499,63 @@ val eval_call_nested_seq_impl_only_tac =
      match_mp_tac call_preserve_state_code_locals_rel >>
      fs [])
 
-val abc_tac =
+val eval_call_append_code_impl_only_tac =
+     qpat_x_assum ‘SOME (Label fname) = eval t x0’ (assume_tac o GSYM) >>
+     qmatch_goalsub_abbrev_tac ‘evaluate (Seq (AppCode x0 ar) pc, _)’ >>
+     drule evaluate_append_code_intro >>
+     fs [panSemTheory.lookup_code_def, CaseEq "option", CaseEq "prod"] >> rveq >>
+     drule code_rel_imp >>
+     disch_then drule >>
+     strip_tac >> fs [] >>
+     fs [lookup_code_def] >>
+     drule (INST_TYPE [``:'c``|->``:num``] list_rel_length_shape_of_flatten) >>
+     disch_then (qspec_then ‘ns’ mp_tac) >>
+     fs [] >> strip_tac >>
+     disch_then (qspecl_then [‘pc’, ‘ar’] assume_tac) >>
+     fs [] >> pop_assum kall_tac >>
+     qmatch_goalsub_abbrev_tac ‘evaluate (_, tnew)’ >>
+     fs [Abbr ‘pc’, evaluate_def] >>
+     ‘eval tnew x0 = eval t x0’ by (
+       fs [Abbr ‘tnew’] >>
+       match_mp_tac eval_upde_code_eq >> fs []) >>
+     fs [] >>
+     ‘OPT_MMAP (eval t)
+      (FLAT (MAP FST (MAP (compile_exp ctxt) argexps))) = SOME (FLAT (MAP flatten args))’ by (
+       fs [opt_mmap_eq_some] >> metis_tac [eval_map_comp_exp_flat_eq]) >>
+     qmatch_asmsub_abbrev_tac ‘t.code |+ (fname,ns,nc)’ >>
+     drule opt_mmap_eval_upde_code_eq >>
+     disch_then (qspecl_then [‘fname’, ‘ns’, ‘nc’] assume_tac) >>
+     fs [Abbr ‘tnew’, lookup_code_def, FLOOKUP_UPDATE] >>
+     drule (INST_TYPE [``:'c``|->``:num``] list_rel_length_shape_of_flatten) >>
+     disch_then (qspec_then ‘ns’ mp_tac) >>
+     fs [FLOOKUP_UPDATE] >>
+     ‘t.clock <> 0’ by fs [state_rel_def] >> fs [] >>
+     cases_on ‘ t.clock = 0’ >- fs [state_rel_def] >>
+     fs [] >> rveq >>
+     fs [Abbr ‘nc’, evaluate_def] >> pairarg_tac >> fs [] >>
+     qmatch_asmsub_abbrev_tac ‘compile_prog nctxt _,nt’ >>
+     last_x_assum (qspecl_then [‘nt’, ‘nctxt’] mp_tac) >>
+     impl_tac
+     >- (
+      (* nasty hack *)
+      ‘state_rel
+         (dec_clock s with locals := FEMPTY |++ ZIP (MAP FST vshapes,args))
+         (dec_clock t with locals := FEMPTY |++ ZIP (ns,FLAT (MAP flatten args))) ∧
+       code_rel nctxt (dec_clock s).code
+         (dec_clock t with locals := FEMPTY |++ ZIP (ns,FLAT (MAP flatten args))).code ∧
+       excp_rel nctxt (dec_clock s).eshapes
+         (dec_clock t with locals := FEMPTY |++ ZIP (ns,FLAT (MAP flatten args))).eids ∧
+       locals_rel nctxt (FEMPTY |++ ZIP (MAP FST vshapes,args))
+         (dec_clock t with locals := FEMPTY |++ ZIP (ns,FLAT (MAP flatten args))).locals’ by (
+        fs [Abbr ‘nctxt’, slc_tlc_rw] >>
+        match_mp_tac call_preserve_state_code_locals_rel >>
+        fs []) >>
+      fs [Abbr ‘nt’,dec_clock_def, state_rel_def, excp_rel_def] >>
+      cheat (*need to update code rel *))
+
+
+
+ val abc_tac =
   rpt gen_tac >> rpt strip_tac >>
   fs [panSemTheory.evaluate_def] >>
   fs [compile_prog_def] >>
@@ -4342,8 +4565,8 @@ val abc_tac =
   drule compile_exp_val_rel >>
   disch_then drule_all >>
   strip_tac >> fs [flatten_def] >> rveq >>
-  cases_on ‘s.clock = 0’ >> fs [] >> rveq >- cheat
- (* >- (
+  cases_on ‘s.clock = 0’ >> fs [] >> rveq
+  >- (
    TOP_CASE_TAC >> fs [] >> rveq
    >- clock_zero_tail_rt_tac
    >- (
@@ -4375,10 +4598,19 @@ val abc_tac =
    TOP_CASE_TAC >> fs []
    >- (
     TOP_CASE_TAC >> fs []
-    >- clock_zero_tail_rt_tac >>
+    >- (
+     TOP_CASE_TAC >> fs []
+     >- clock_zero_tail_rt_tac >>
+     TOP_CASE_TAC >> fs [] >>
+     TOP_CASE_TAC >> fs []
+     >- (
+      TOP_CASE_TAC >> fs []
+      >- clock_zero_tail_rt_tac >>
+      clock_zero_tail_rt_tac) >>
+     TOP_CASE_TAC >> fs []
+     >- clock_zero_tail_rt_tac >>
+     clock_zero_nested_seq_rt_tac) >>
     TOP_CASE_TAC >> fs [] >>
-    TOP_CASE_TAC >> fs []
-    >- clock_zero_tail_rt_tac >>
     TOP_CASE_TAC >> fs []
     >- (
      TOP_CASE_TAC >> fs []
@@ -4392,8 +4624,31 @@ val abc_tac =
      TOP_CASE_TAC >> fs []
      >- clock_zero_tail_rt_tac >>
      clock_zero_nested_seq_rt_tac) >>
-    clock_zero_tail_rt_tac) >>
-   clock_zero_tail_rt_tac) *) >>
+    TOP_CASE_TAC >> fs []
+    >- (
+     TOP_CASE_TAC >> fs []
+     >- clock_zero_tail_rt_tac >>
+     TOP_CASE_TAC >> fs [] >>
+     TOP_CASE_TAC >> fs []
+     >- (
+      TOP_CASE_TAC >> fs []
+      >- clock_zero_tail_rt_tac >>
+      clock_zero_tail_rt_tac) >>
+     TOP_CASE_TAC >> fs []
+     >- clock_zero_tail_rt_tac >>
+     clock_zero_append_code_tac) >>
+    TOP_CASE_TAC >> fs []
+    >- clock_zero_tail_rt_tac >>
+    TOP_CASE_TAC >> fs [] >>
+    TOP_CASE_TAC >> fs []
+    >- (
+     TOP_CASE_TAC >> fs []
+     >- clock_zero_tail_rt_tac >>
+     clock_zero_tail_rt_tac) >>
+    TOP_CASE_TAC >> fs []
+    >- clock_zero_tail_rt_tac >>
+    clock_zero_nested_seq_rt_tac) >>
+   cheat) >>
   (* s <> 0 case *)
   TOP_CASE_TAC >> fs []
   >- (
@@ -4488,8 +4743,7 @@ val abc_tac =
      conj_tac
      >- (
       fs [excp_rel_def, ctxt_fc_code_vars_eq,ctxt_fc_eid_map_eq,
-          panSemTheory.set_var_def,set_var_def] >> rw [] >>
-      res_tac >> fs []) >>
+          panSemTheory.set_var_def,set_var_def]) >>
      ‘size_of_shape (shape_of v) = 1’ by fs [] >>
       drule locals_rel_lookup_ctxt >>
       disch_then drule >> strip_tac >> fs [] >>
@@ -4528,8 +4782,7 @@ val abc_tac =
      conj_tac
      >- (
       fs [excp_rel_def, ctxt_fc_code_vars_eq,ctxt_fc_eid_map_eq,
-          panSemTheory.set_var_def,set_var_def] >> rw [] >>
-      res_tac >> fs []) >>
+          panSemTheory.set_var_def,set_var_def]) >>
      ‘size_of_shape (shape_of v) = 1’ by fs [] >>
       drule locals_rel_lookup_ctxt >>
       disch_then drule >> strip_tac >> fs [] >>
@@ -4586,8 +4839,7 @@ val abc_tac =
      conj_tac >- fs [Abbr ‘nctxt’, code_rel_def, ctxt_fc_code_vars_eq, ctxt_fc_eid_map_eq] >>
      conj_tac
      >- (
-      fs [Abbr ‘nctxt’, excp_rel_def, ctxt_fc_code_vars_eq, ctxt_fc_eid_map_eq] >>
-      rw [] >> last_x_assum drule_all >> fs []) >>
+      fs [Abbr ‘nctxt’, excp_rel_def, ctxt_fc_code_vars_eq, ctxt_fc_eid_map_eq]) >>
      fs [locals_rel_def] >> rw [] >>
      fs [FLOOKUP_UPDATE] >> FULL_CASE_TAC >> fs [] >> rveq
      >- (
@@ -4645,8 +4897,7 @@ val abc_tac =
     conj_tac >- fs [Abbr ‘nctxt’, code_rel_def, ctxt_fc_code_vars_eq, ctxt_fc_eid_map_eq] >>
     conj_tac
     >- (
-     fs [Abbr ‘nctxt’, excp_rel_def, ctxt_fc_code_vars_eq, ctxt_fc_eid_map_eq] >>
-     rw [] >>last_x_assum drule_all >> fs []) >>
+     fs [Abbr ‘nctxt’, excp_rel_def, ctxt_fc_code_vars_eq, ctxt_fc_eid_map_eq]) >>
     ‘MAP (λn. THE (FLOOKUP t1.globals n)) (GENLIST (λx. n2w x) (LENGTH r')) =
      flatten v’ by (
       fs [opt_mmap_eq_some] >>
@@ -4660,234 +4911,130 @@ val abc_tac =
     match_mp_tac local_rel_le_zip_update_preserved >> fs [] >>
     match_mp_tac local_rel_gt_max_var_preserved >>
     fs [])
-   >- cheat >>
+   >- (  (* exception value with ret call *)
+    TOP_CASE_TAC >> fs []
+    >- (
+     eval_call_impl_only_tac >>
+     strip_tac >> fs [] >>
+     ‘nctxt.eid_map = ctxt.eid_map’ by
+       fs [Abbr ‘nctxt’, ctxt_fc_eid_map_eq] >>
+     cases_on ‘FLOOKUP ctxt.eid_map m'’ >> fs [] >>
+     cases_on ‘x’ >> fs [] >>
+     cases_on ‘size_of_shape (shape_of v) = 0’ >> fs []
+     >- rels_empty_tac >>
+     cases_on ‘size_of_shape (shape_of v) = 1’ >> fs []
+     >- (fs [shape_of_def, panLangTheory.size_of_shape_def] >> rels_empty_tac) >>
+     rels_empty_tac) >>
+    TOP_CASE_TAC >> fs [] >>
+    TOP_CASE_TAC >> fs []
+    >- (
+     TOP_CASE_TAC >> fs []
+     >- (
+      eval_call_impl_only_tac >>
+      strip_tac >> fs [] >>
+      ‘nctxt.eid_map = ctxt.eid_map’ by
+        fs [Abbr ‘nctxt’, ctxt_fc_eid_map_eq] >>
+      cases_on ‘FLOOKUP ctxt.eid_map m'’ >> fs [] >>
+      cases_on ‘x’ >> fs [] >>
+      cases_on ‘size_of_shape (shape_of v) = 0’ >> fs []
+      >- rels_empty_tac >>
+      cases_on ‘size_of_shape (shape_of v) = 1’ >> fs []
+      >- (fs [shape_of_def, panLangTheory.size_of_shape_def] >> rels_empty_tac) >>
+      rels_empty_tac) >>
+     eval_call_impl_only_tac >>
+     strip_tac >> fs [] >>
+     ‘nctxt.eid_map = ctxt.eid_map’ by
+       fs [Abbr ‘nctxt’, ctxt_fc_eid_map_eq] >>
+     cases_on ‘FLOOKUP ctxt.eid_map m'’ >> fs [] >>
+     cases_on ‘x’ >> fs [] >>
+     cases_on ‘size_of_shape (shape_of v) = 0’ >> fs []
+     >- rels_empty_tac >>
+     cases_on ‘size_of_shape (shape_of v) = 1’ >> fs []
+     >- (fs [shape_of_def, panLangTheory.size_of_shape_def] >> rels_empty_tac) >>
+     rels_empty_tac) >>
+    TOP_CASE_TAC >> fs []
+    >- (
+     eval_call_impl_only_tac >>
+     strip_tac >> fs [] >>
+     ‘nctxt.eid_map = ctxt.eid_map’ by
+       fs [Abbr ‘nctxt’, ctxt_fc_eid_map_eq] >>
+     cases_on ‘FLOOKUP ctxt.eid_map m'’ >> fs [] >>
+     cases_on ‘x’ >> fs [] >>
+     cases_on ‘size_of_shape (shape_of v) = 0’ >> fs []
+     >- rels_empty_tac >>
+     cases_on ‘size_of_shape (shape_of v) = 1’ >> fs []
+     >- (fs [shape_of_def, panLangTheory.size_of_shape_def] >> rels_empty_tac) >>
+     rels_empty_tac) >>
+    eval_call_nested_seq_impl_only_tac >>
+    strip_tac >> fs [] >>
+    ‘nctxt.eid_map = ctxt.eid_map’ by
+      fs [Abbr ‘nctxt’, ctxt_fc_eid_map_eq] >>
+    cases_on ‘FLOOKUP ctxt.eid_map m'’ >> fs [] >>
+    cases_on ‘x’ >> fs [] >>
+    cases_on ‘res1’ >> fs [] >> rveq >> fs [] >>
+    TRY (cases_on ‘x’ >> fs [] >> rveq >> fs []) >>
+    cases_on ‘FLOOKUP ctxt.eid_map m'’ >> fs [] >>
+    cases_on ‘x’ >> fs [] >>
+    cases_on ‘size_of_shape (shape_of v) = 0’ >> fs []
+    >- rels_empty_tac >>
+    cases_on ‘size_of_shape (shape_of v) = 1’ >> fs []
+    >- (
+     fs [shape_of_def, panLangTheory.size_of_shape_def] >>
+     rels_empty_tac) >>
+    rels_empty_tac) >>
    TOP_CASE_TAC
    >- call_tail_ret_impl_tac >>
    TOP_CASE_TAC  >> TOP_CASE_TAC
    >- (
-    TOP_CASE_TAC >- call_tail_ret_impl_tac >>
+    TOP_CASE_TAC
+    >- call_tail_ret_impl_tac >>
     call_tail_ret_impl_tac) >>
    TOP_CASE_TAC >> fs []
    >- call_tail_ret_impl_tac >>
    call_nested_seq_ret_impl_tac)
 
-
 val handle_ret_time_out_case =
+     TOP_CASE_TAC >> fs []
+     >- call_tail_ret_impl_tac >>
+     TOP_CASE_TAC >> fs [] >>
+     TOP_CASE_TAC >> fs []
+     >- (
       TOP_CASE_TAC >> fs []
       >- call_tail_ret_impl_tac >>
-      TOP_CASE_TAC >> fs [] >>
-      TOP_CASE_TAC >> fs []
-      >- (
-       TOP_CASE_TAC >> fs []
-       >- call_tail_ret_impl_tac >>
-       call_tail_ret_impl_tac) >>
-      TOP_CASE_TAC >> fs []
-      >- call_tail_ret_impl_tac >>
-      call_nested_seq_ret_impl_tac
+      call_tail_ret_impl_tac) >>
+     TOP_CASE_TAC >> fs []
+     >- call_tail_ret_impl_tac >>
+     call_nested_seq_ret_impl_tac
 
-val handle_ret_ret_case =
-      rename [‘is_valid_value s.locals m v’] >>
-      fs [is_valid_value_def] >>
-      cases_on ‘FLOOKUP s.locals m’ >> fs [] >>
+val time_out_handle_tac =  (*Time out case *)
+    TOP_CASE_TAC >> fs []
+    >- handle_ret_time_out_case >>
+    rename [‘FLOOKUP ctxt.var_nums evar’] >>
+    TOP_CASE_TAC >> fs [] >>
+    TOP_CASE_TAC >> fs []
+    >- ((* lookup eid = SOME (One, _) *)
+     TOP_CASE_TAC >> fs []
+     >- handle_ret_time_out_case >>
+     TOP_CASE_TAC >> fs [] >>
+     TOP_CASE_TAC >> fs []
+     >- handle_ret_time_out_case >>
+     reverse TOP_CASE_TAC >> fs []
+     >- handle_ret_time_out_case >>
+     TOP_CASE_TAC >> fs []
+     >- call_tail_ret_impl_tac >>
+     TOP_CASE_TAC >> fs [] >>
+     TOP_CASE_TAC >> fs []
+     >- (
       TOP_CASE_TAC >> fs []
-      >- (fs [locals_rel_def] >> first_x_assum drule >> fs []) >>
-      TOP_CASE_TAC >> fs [] >>
-      TOP_CASE_TAC >> fs []
-      >- (
-       TOP_CASE_TAC >> fs []
-       >- (
-        fs [locals_rel_def] >> first_x_assum drule >> fs [] >>
-        fs [OPT_MMAP_def] >>
-        strip_tac >> fs [] >>
-        pop_assum (assume_tac o GSYM) >>
-        ‘size_of_shape (shape_of x) = 1’ by
-          fs [panLangTheory.size_of_shape_def, shape_of_def] >>
-        fs [GSYM length_flatten_eq_size_of_shape] >> rfs [flatten_def]) >>
-       eval_call_impl_only_tac >>
-       strip_tac >> fs [] >>
-       ‘size_of_shape (shape_of x) = 1’ by (
-         fs [locals_rel_def] >>
-         last_x_assum drule >>
-         fs [shape_of_def]) >>
-       fs [shape_of_def] >>
-       fs [state_rel_def, panSemTheory.set_var_def,set_var_def,
-           Abbr ‘nctxt’, code_rel_def, ctxt_fc_code_vars_eq,ctxt_fc_eid_map_eq,
-           panSemTheory.set_var_def,set_var_def] >>
-       conj_tac
-       >- (
-        fs [excp_rel_def, ctxt_fc_code_vars_eq,ctxt_fc_eid_map_eq,
-            panSemTheory.set_var_def,set_var_def] >> rw [] >>
-        res_tac >> fs []) >>
-       ‘size_of_shape (shape_of v) = 1’ by fs [] >>
-       drule locals_rel_lookup_ctxt >>
-       disch_then drule >> strip_tac >> fs [] >>
-       rveq >> fs [length_flatten_eq_size_of_shape] >>
-       rfs [panLangTheory.size_of_shape_def] >>
-       fs [locals_rel_def, panSemTheory.set_var_def,set_var_def] >>
-       rw [] >> rveq >>
-       fs [FLOOKUP_UPDATE] >>
-       FULL_CASE_TAC >> fs [] >> rveq
-       >- (
-        fs [OPT_MMAP_def, FLOOKUP_UPDATE] >> rveq >>
-        fs [length_flatten_eq_size_of_shape, panLangTheory.size_of_shape_def]) >>
-       res_tac >> fs [] >>
-       match_mp_tac opt_mmap_flookup_update >>
-       fs [] >>
-       drule no_overlap_flookup_distinct >>
-       disch_then drule_all >> fs [distinct_lists_def]) >>
-      TOP_CASE_TAC >> fs []
-      >- (
-       ‘LENGTH r'' = 1’ by (
-         drule_all locals_rel_lookup_ctxt >> strip_tac >>
-         fs [length_flatten_eq_size_of_shape] >>
-         rfs [panLangTheory.size_of_shape_def]) >>
-       fs [] >>
-       cases_on ‘r''’ >> fs [ooHD_def] >>
-       eval_call_impl_only_tac >>
-       strip_tac >> fs [] >>
-       ‘size_of_shape (shape_of x) = 1’ by (
-         drule_all locals_rel_lookup_ctxt >> strip_tac >>
-         fs [length_flatten_eq_size_of_shape] >>
-         rfs [panLangTheory.size_of_shape_def]) >>
-       fs [shape_of_def, panLangTheory.size_of_shape_def] >>
-       fs [state_rel_def, panSemTheory.set_var_def,set_var_def,
-           Abbr ‘nctxt’, code_rel_def, ctxt_fc_code_vars_eq,ctxt_fc_eid_map_eq,
-           panSemTheory.set_var_def,set_var_def] >>
-       conj_tac
-       >- (
-        fs [excp_rel_def, ctxt_fc_code_vars_eq,ctxt_fc_eid_map_eq,
-            panSemTheory.set_var_def,set_var_def] >> rw [] >>
-        res_tac >> fs []) >>
-       ‘size_of_shape (shape_of v) = 1’ by fs [] >>
-       drule locals_rel_lookup_ctxt >>
-       disch_then drule >> strip_tac >> fs [] >>
-       rveq >> fs [length_flatten_eq_size_of_shape] >>
-       rfs [panLangTheory.size_of_shape_def] >>
-       fs [locals_rel_def, panSemTheory.set_var_def,set_var_def] >>
-       rw [] >> rveq >>
-       fs [FLOOKUP_UPDATE] >>
-       FULL_CASE_TAC >> fs [] >> rveq
-       >- (
-        fs [OPT_MMAP_def, FLOOKUP_UPDATE] >> rveq >>
-        fs [length_flatten_eq_size_of_shape, panLangTheory.size_of_shape_def]) >>
-       res_tac >> fs [] >>
-       match_mp_tac opt_mmap_flookup_update >>
-       fs [] >>
-       drule no_overlap_flookup_distinct >>
-       disch_then drule_all >> fs [distinct_lists_def]) >>
-      fs [nested_seq_def, evaluate_def] >> pairarg_tac >> fs [] >>
-      cases_on ‘eval t x0’ >> fs [] >>
-      cases_on ‘x'’ >> fs [] >>
-      ‘OPT_MMAP (eval t)
-       (FLAT (MAP FST (MAP (compile_exp ctxt) argexps))) = SOME (FLAT (MAP flatten args))’ by (
-        fs [opt_mmap_eq_some] >> metis_tac [eval_map_comp_exp_flat_eq]) >>
-      fs [] >>
-      fs [panSemTheory.lookup_code_def, CaseEq "option", CaseEq "prod"] >> rveq >>
-      drule code_rel_imp >>
-      disch_then drule >>
-      strip_tac >> fs [] >>
-      fs [lookup_code_def] >>
-      drule (INST_TYPE [``:'c``|->``:num``] list_rel_length_shape_of_flatten) >>
-      disch_then (qspec_then ‘ns’ mp_tac) >>
-      fs [] >>
-      cases_on ‘ t.clock = 0’ >- fs [state_rel_def] >>
-      fs [] >> rveq >>
-      qmatch_asmsub_abbrev_tac ‘compile_prog nctxt _,nt’ >>
-      first_x_assum (qspecl_then [‘nt’, ‘nctxt’] mp_tac) >>
-      impl_tac
-      >- (
-       fs [Abbr ‘nctxt’, Abbr ‘nt’, slc_tlc_rw] >>
-       match_mp_tac call_preserve_state_code_locals_rel >>
-       fs []) >>
-      strip_tac >> fs [] >>
-      cases_on ‘res1’ >> fs [] >>
-      cases_on ‘x'’ >> fs [] >> rveq >> fs [] >>
-      fs [shape_of_def, panLangTheory.size_of_shape_def,
-          panSemTheory.set_var_def, set_var_def] >>
-      cases_on ‘size_of_shape (shape_of x) = 0’ >> fs []
-      >- (
-       rveq >> drule locals_rel_lookup_ctxt >>
-       disch_then (qspecl_then [‘m’, ‘x’] assume_tac) >>
-       fs [length_flatten_eq_size_of_shape] >> rfs [] >> rveq >>
-       fs [nested_seq_def, evaluate_def] >>
-       conj_tac >- fs [state_rel_def] >>
-       conj_tac >- fs [Abbr ‘nctxt’, code_rel_def, ctxt_fc_code_vars_eq, ctxt_fc_eid_map_eq] >>
-       conj_tac
-       >- (
-        fs [Abbr ‘nctxt’, excp_rel_def, ctxt_fc_code_vars_eq, ctxt_fc_eid_map_eq] >>
-        rw [] >> last_x_assum drule_all >> fs []) >>
-       fs [locals_rel_def] >> rw [] >>
-       fs [FLOOKUP_UPDATE] >> FULL_CASE_TAC >> fs [] >> rveq
-       >- (
-        fs [OPT_MMAP_def] >>
-        ‘LENGTH (flatten v) = 0’ suffices_by fs[] >>
-        rewrite_tac [length_flatten_eq_size_of_shape] >>
-        fs []) >>
-       first_x_assum drule >> strip_tac >> fs [] >>
-       fs [opt_mmap_eq_some, MAP_EQ_EVERY2, LIST_REL_EL_EQN] >>
-       rw [] >> fs [FLOOKUP_UPDATE] >>
-       TOP_CASE_TAC >> fs [] >>
-       drule ctxt_max_el_leq >>
-       qpat_x_assum ‘LENGTH _ = LENGTH (flatten _)’ (assume_tac o GSYM) >>
-       fs [] >> disch_then drule_all >> fs []) >>
-      ‘1 < size_of_shape (shape_of x)’ by (
-        drule locals_rel_lookup_ctxt >>
-        disch_then drule >>
-        strip_tac >> fs [] >> rfs [] >>
-        fs [panLangTheory.size_of_shape_def] >>
-        DECIDE_TAC) >>
-      fs [] >>
-      ‘ALL_DISTINCT r''’ by
-        (fs [locals_rel_def] >> imp_res_tac all_distinct_flookup_all_distinct) >>
-      fs [globals_lookup_def] >>
-      drule evaluate_seq_assign_load_globals >>
-      disch_then (qspecl_then [‘t1 with locals :=
-                                t.locals |+ (ctxt.max_var + 1,Word 0w)’, ‘0w’] mp_tac) >>
-      impl_tac
-      >- (
-       conj_tac
-       >- (
-        fs [word_0_n2w] >>
-        imp_res_tac locals_rel_lookup_ctxt >> rveq >>
-        fs [length_flatten_eq_size_of_shape] >> rfs []) >>
-       conj_tac
-       >- (
-        rw [] >>
-        ‘n <> ctxt.max_var + 1’ suffices_by (
-                                fs [FLOOKUP_UPDATE, locals_rel_def] >>
-                                first_x_assum drule_all >> strip_tac >> fs [] >> rveq >>
-                                imp_res_tac opt_mmap_mem_func >> fs []) >>
-        fs [locals_rel_def, ctxt_max_def] >>
-        last_x_assum drule_all >> strip_tac >> fs []) >>
-       rw [] >> rfs [] >>
-       drule locals_rel_lookup_ctxt >>
-       ‘size_of_shape (shape_of x) = LENGTH r''’ by (
-         drule locals_rel_lookup_ctxt >>
-         disch_then drule >>
-         strip_tac >> fs [] >> rveq >>
-         fs [length_flatten_eq_size_of_shape] >> rfs []) >>
-       fs [] >> drule opt_mmap_mem_func >>
-       disch_then drule >> strip_tac >> fs []) >>
-      strip_tac >> fs [] >>
-      conj_tac >- fs [state_rel_def] >>
-      conj_tac >- fs [Abbr ‘nctxt’, code_rel_def, ctxt_fc_code_vars_eq, ctxt_fc_eid_map_eq] >>
-      conj_tac
-      >- (
-       fs [Abbr ‘nctxt’, excp_rel_def, ctxt_fc_code_vars_eq, ctxt_fc_eid_map_eq] >>
-       rw [] >>last_x_assum drule_all >> fs []) >>
-      ‘MAP (λn. THE (FLOOKUP t1.globals n)) (GENLIST (λx. n2w x) (LENGTH r'')) =
-       flatten v’ by (
-        fs [opt_mmap_eq_some] >>
-        ‘size_of_shape (shape_of v) = LENGTH r''’ by (
-          drule locals_rel_lookup_ctxt >>
-          disch_then drule >>
-          strip_tac >> fs [] >> rveq >>
-          fs [length_flatten_eq_size_of_shape] >> rfs []) >>
-        fs [] >> drule map_some_the_map >> fs []) >>
-      fs [] >>
-      match_mp_tac local_rel_le_zip_update_preserved >> fs [] >>
-      match_mp_tac local_rel_gt_max_var_preserved >>
-      fs []
+      >- call_tail_ret_impl_tac >>
+      call_tail_ret_impl_tac) >>
+     TOP_CASE_TAC >> fs []
+     >- call_tail_ret_impl_tac >>
+     eval_call_append_code_impl_only_tac >>
+     fs [] >> strip_tac >>
+     fs [Abbr ‘nctxt’, state_rel_def, ctxt_fc_code_vars_eq, ctxt_fc_eid_map_eq,
+         empty_locals_def, panSemTheory.empty_locals_def, code_rel_def, ctxt_fc_eid_map_eq, excp_rel_def]) >>
+    cheat  (* the comb eid case *)
 
 val eid_none_ret_handle_case =
      TOP_CASE_TAC >> fs []
@@ -4921,8 +5068,7 @@ val eid_none_ret_handle_case =
       conj_tac
       >- (
        fs [excp_rel_def, ctxt_fc_code_vars_eq,ctxt_fc_eid_map_eq,
-           panSemTheory.set_var_def,set_var_def] >> rw [] >>
-       res_tac >> fs []) >>
+           panSemTheory.set_var_def,set_var_def]) >>
       ‘size_of_shape (shape_of v) = 1’ by fs [] >>
       drule locals_rel_lookup_ctxt >>
       disch_then drule >> strip_tac >> fs [] >>
@@ -4963,8 +5109,7 @@ val eid_none_ret_handle_case =
       conj_tac
       >- (
        fs [excp_rel_def, ctxt_fc_code_vars_eq,ctxt_fc_eid_map_eq,
-           panSemTheory.set_var_def,set_var_def] >> rw [] >>
-       res_tac >> fs []) >>
+           panSemTheory.set_var_def,set_var_def]) >>
       ‘size_of_shape (shape_of v) = 1’ by fs [] >>
       drule locals_rel_lookup_ctxt >>
       disch_then drule >> strip_tac >> fs [] >>
@@ -5023,8 +5168,7 @@ val eid_none_ret_handle_case =
       conj_tac >- fs [Abbr ‘nctxt’, code_rel_def, ctxt_fc_code_vars_eq, ctxt_fc_eid_map_eq] >>
       conj_tac
       >- (
-       fs [Abbr ‘nctxt’, excp_rel_def, ctxt_fc_code_vars_eq, ctxt_fc_eid_map_eq] >>
-       rw [] >> last_x_assum drule_all >> fs []) >>
+       fs [Abbr ‘nctxt’, excp_rel_def, ctxt_fc_code_vars_eq, ctxt_fc_eid_map_eq]) >>
       fs [locals_rel_def] >> rw [] >>
       fs [FLOOKUP_UPDATE] >> FULL_CASE_TAC >> fs [] >> rveq
       >- (
@@ -5084,8 +5228,7 @@ val eid_none_ret_handle_case =
      conj_tac >- fs [Abbr ‘nctxt’, code_rel_def, ctxt_fc_code_vars_eq, ctxt_fc_eid_map_eq] >>
      conj_tac
      >- (
-      fs [Abbr ‘nctxt’, excp_rel_def, ctxt_fc_code_vars_eq, ctxt_fc_eid_map_eq] >>
-      rw [] >>last_x_assum drule_all >> fs []) >>
+      fs [Abbr ‘nctxt’, excp_rel_def, ctxt_fc_code_vars_eq, ctxt_fc_eid_map_eq]) >>
      ‘MAP (λn. THE (FLOOKUP t1.globals n)) (GENLIST (λx. n2w x) (LENGTH r')) =
       flatten v’ by (
        fs [opt_mmap_eq_some] >>
@@ -5100,68 +5243,208 @@ val eid_none_ret_handle_case =
      match_mp_tac local_rel_gt_max_var_preserved >>
      fs []
 
-
-Theorem max_set_list_max:
-  !xs. MAX_SET (set xs) = list_max xs
-Proof
-  Induct >> rw [] >> fs [list_max_def] >>
-  ‘FINITE (set xs)’ by fs [] >>
-  drule (MAX_SET_THM |> CONJUNCT2) >>
-  disch_then (qspec_then ‘h’ assume_tac) >>
-  fs [] >>
-  TOP_CASE_TAC >>fs [MAX_DEF]
-QED
-
-
-Theorem list_max_add_not_mem:
-  !xs. ~MEM (list_max xs + 1) xs
-Proof
-  Induct >> rw [] >> fs [list_max_def] >>
-  CCONTR_TAC >> fs [] >>
-  every_case_tac >> fs [list_max_def] >>
-  ntac 2 (pop_assum mp_tac) >> pop_assum kall_tac >>
-  qid_spec_tac ‘xs’ >>
-  Induct >> rw [] >> fs [list_max_def]
-QED
-
-
-
-Theorem compile_Call:
-  ^(get_goal "compile_prog _ (panLang$Call _ _ _)")
-Proof
-   abc_tac >>
-   (* Handler case *)
-   rename [‘FLOOKUP ctxt.eid_map eid’] >>
-   cases_on ‘evaluate (prog,dec_clock s with locals := newlocals)’ >>
-   fs [] >> cases_on ‘q’ >> fs [] >> cases_on ‘x’ >> fs []
-   >- ( (*Time out case *)
-    TOP_CASE_TAC >> fs []
-    >- ( (* lookup eid = NONE *)
-     TOP_CASE_TAC >> fs []
-     >- call_tail_ret_impl_tac >>
-     TOP_CASE_TAC >> fs [] >>
-     TOP_CASE_TAC >> fs []
-     >- (
+val handle_ret_ret_case =
+      rename [‘is_valid_value s.locals m v’] >>
+      fs [is_valid_value_def] >>
+      cases_on ‘FLOOKUP s.locals m’ >> fs [] >>
       TOP_CASE_TAC >> fs []
-      >- call_tail_ret_impl_tac >>
-      call_tail_ret_impl_tac) >>
-     TOP_CASE_TAC >> fs []
-     >- call_tail_ret_impl_tac >>
-     call_nested_seq_ret_impl_tac) >>
-    rename [‘FLOOKUP ctxt.var_nums evar’] >>
-    TOP_CASE_TAC >> fs [] >>
-    TOP_CASE_TAC >> fs []
-    >- ((* lookup eid = SOME (One, _) *)
-     TOP_CASE_TAC >> fs []
-     >- handle_ret_time_out_case >>
-     TOP_CASE_TAC >> fs [] >>
-     TOP_CASE_TAC >> fs []
-     >- handle_ret_time_out_case >>
-     TOP_CASE_TAC >> fs []
-     >- handle_ret_time_out_case >>
-     handle_ret_time_out_case) >>
-    cheat) (* the comb eid case *)
-   >- ( (* Return case *)
+      >- (fs [locals_rel_def] >> first_x_assum drule >> fs []) >>
+      TOP_CASE_TAC >> fs [] >>
+      TOP_CASE_TAC >> fs []
+      >- (
+       TOP_CASE_TAC >> fs []
+       >- (
+        fs [locals_rel_def] >> first_x_assum drule >> fs [] >>
+        fs [OPT_MMAP_def] >>
+        strip_tac >> fs [] >>
+        pop_assum (assume_tac o GSYM) >>
+        ‘size_of_shape (shape_of x) = 1’ by
+          fs [panLangTheory.size_of_shape_def, shape_of_def] >>
+        fs [GSYM length_flatten_eq_size_of_shape] >> rfs [flatten_def]) >>
+       eval_call_impl_only_tac >>
+       strip_tac >> fs [] >>
+       ‘size_of_shape (shape_of x) = 1’ by (
+         fs [locals_rel_def] >>
+         last_x_assum drule >>
+         fs [shape_of_def]) >>
+       fs [shape_of_def] >>
+       fs [state_rel_def, panSemTheory.set_var_def,set_var_def,
+           Abbr ‘nctxt’, code_rel_def, ctxt_fc_code_vars_eq,ctxt_fc_eid_map_eq,
+           panSemTheory.set_var_def,set_var_def] >>
+       conj_tac
+       >- (
+        fs [excp_rel_def, ctxt_fc_code_vars_eq,ctxt_fc_eid_map_eq,
+            panSemTheory.set_var_def,set_var_def]) >>
+       ‘size_of_shape (shape_of v) = 1’ by fs [] >>
+       drule locals_rel_lookup_ctxt >>
+       disch_then drule >> strip_tac >> fs [] >>
+       rveq >> fs [length_flatten_eq_size_of_shape] >>
+       rfs [panLangTheory.size_of_shape_def] >>
+       fs [locals_rel_def, panSemTheory.set_var_def,set_var_def] >>
+       rw [] >> rveq >>
+       fs [FLOOKUP_UPDATE] >>
+       FULL_CASE_TAC >> fs [] >> rveq
+       >- (
+        fs [OPT_MMAP_def, FLOOKUP_UPDATE] >> rveq >>
+        fs [length_flatten_eq_size_of_shape, panLangTheory.size_of_shape_def]) >>
+       res_tac >> fs [] >>
+       match_mp_tac opt_mmap_flookup_update >>
+       fs [] >>
+       drule no_overlap_flookup_distinct >>
+       disch_then drule_all >> fs [distinct_lists_def]) >>
+      TOP_CASE_TAC >> fs []
+      >- (
+       ‘LENGTH r'' = 1’ by (
+         drule_all locals_rel_lookup_ctxt >> strip_tac >>
+         fs [length_flatten_eq_size_of_shape] >>
+         rfs [panLangTheory.size_of_shape_def]) >>
+       fs [] >>
+       cases_on ‘r''’ >> fs [ooHD_def] >>
+       eval_call_impl_only_tac >>
+       strip_tac >> fs [] >>
+       ‘size_of_shape (shape_of x) = 1’ by (
+         drule_all locals_rel_lookup_ctxt >> strip_tac >>
+         fs [length_flatten_eq_size_of_shape] >>
+         rfs [panLangTheory.size_of_shape_def]) >>
+       fs [shape_of_def, panLangTheory.size_of_shape_def] >>
+       fs [state_rel_def, panSemTheory.set_var_def,set_var_def,
+           Abbr ‘nctxt’, code_rel_def, ctxt_fc_code_vars_eq,ctxt_fc_eid_map_eq,
+           panSemTheory.set_var_def,set_var_def] >>
+       conj_tac
+       >- (
+        fs [excp_rel_def, ctxt_fc_code_vars_eq,ctxt_fc_eid_map_eq,
+            panSemTheory.set_var_def,set_var_def]) >>
+       ‘size_of_shape (shape_of v) = 1’ by fs [] >>
+       drule locals_rel_lookup_ctxt >>
+       disch_then drule >> strip_tac >> fs [] >>
+       rveq >> fs [length_flatten_eq_size_of_shape] >>
+       rfs [panLangTheory.size_of_shape_def] >>
+       fs [locals_rel_def, panSemTheory.set_var_def,set_var_def] >>
+       rw [] >> rveq >>
+       fs [FLOOKUP_UPDATE] >>
+       FULL_CASE_TAC >> fs [] >> rveq
+       >- (
+        fs [OPT_MMAP_def, FLOOKUP_UPDATE] >> rveq >>
+        fs [length_flatten_eq_size_of_shape, panLangTheory.size_of_shape_def]) >>
+       res_tac >> fs [] >>
+       match_mp_tac opt_mmap_flookup_update >>
+       fs [] >>
+       drule no_overlap_flookup_distinct >>
+       disch_then drule_all >> fs [distinct_lists_def]) >>
+      fs [nested_seq_def, evaluate_def] >> pairarg_tac >> fs [] >>
+      cases_on ‘eval t x0’ >> fs [] >>
+      cases_on ‘x'’ >> fs [] >>
+      ‘OPT_MMAP (eval t)
+       (FLAT (MAP FST (MAP (compile_exp ctxt) argexps))) = SOME (FLAT (MAP flatten args))’ by (
+        fs [opt_mmap_eq_some] >> metis_tac [eval_map_comp_exp_flat_eq]) >>
+      fs [] >>
+      fs [panSemTheory.lookup_code_def, CaseEq "option", CaseEq "prod"] >> rveq >>
+      drule code_rel_imp >>
+      disch_then drule >>
+      strip_tac >> fs [] >>
+      fs [lookup_code_def] >>
+      drule (INST_TYPE [``:'c``|->``:num``] list_rel_length_shape_of_flatten) >>
+      disch_then (qspec_then ‘ns’ mp_tac) >>
+      fs [] >>
+      cases_on ‘ t.clock = 0’ >- fs [state_rel_def] >>
+      fs [] >> rveq >>
+      qmatch_asmsub_abbrev_tac ‘compile_prog nctxt _,nt’ >>
+      first_x_assum (qspecl_then [‘nt’, ‘nctxt’] mp_tac) >>
+      impl_tac
+      >- (
+       fs [Abbr ‘nctxt’, Abbr ‘nt’, slc_tlc_rw] >>
+       match_mp_tac call_preserve_state_code_locals_rel >>
+       fs []) >>
+      strip_tac >> fs [] >>
+      cases_on ‘res1’ >> fs [] >>
+      cases_on ‘x'’ >> fs [] >> rveq >> fs [] >>
+      fs [shape_of_def, panLangTheory.size_of_shape_def,
+          panSemTheory.set_var_def, set_var_def] >>
+      cases_on ‘size_of_shape (shape_of x) = 0’ >> fs []
+      >- (
+       rveq >> drule locals_rel_lookup_ctxt >>
+       disch_then (qspecl_then [‘m’, ‘x’] assume_tac) >>
+       fs [length_flatten_eq_size_of_shape] >> rfs [] >> rveq >>
+       fs [nested_seq_def, evaluate_def] >>
+       conj_tac >- fs [state_rel_def] >>
+       conj_tac >- fs [Abbr ‘nctxt’, code_rel_def, ctxt_fc_code_vars_eq, ctxt_fc_eid_map_eq] >>
+       conj_tac
+       >- (
+        fs [Abbr ‘nctxt’, excp_rel_def, ctxt_fc_code_vars_eq, ctxt_fc_eid_map_eq]) >>
+       fs [locals_rel_def] >> rw [] >>
+       fs [FLOOKUP_UPDATE] >> FULL_CASE_TAC >> fs [] >> rveq
+       >- (
+        fs [OPT_MMAP_def] >>
+        ‘LENGTH (flatten v) = 0’ suffices_by fs[] >>
+        rewrite_tac [length_flatten_eq_size_of_shape] >>
+        fs []) >>
+       first_x_assum drule >> strip_tac >> fs [] >>
+       fs [opt_mmap_eq_some, MAP_EQ_EVERY2, LIST_REL_EL_EQN] >>
+       rw [] >> fs [FLOOKUP_UPDATE] >>
+       TOP_CASE_TAC >> fs [] >>
+       drule ctxt_max_el_leq >>
+       qpat_x_assum ‘LENGTH _ = LENGTH (flatten _)’ (assume_tac o GSYM) >>
+       fs [] >> disch_then drule_all >> fs []) >>
+      ‘1 < size_of_shape (shape_of x)’ by (
+        drule locals_rel_lookup_ctxt >>
+        disch_then drule >>
+        strip_tac >> fs [] >> rfs [] >>
+        fs [panLangTheory.size_of_shape_def] >>
+        DECIDE_TAC) >>
+      fs [] >>
+      ‘ALL_DISTINCT r''’ by
+        (fs [locals_rel_def] >> imp_res_tac all_distinct_flookup_all_distinct) >>
+      fs [globals_lookup_def] >>
+      drule evaluate_seq_assign_load_globals >>
+      disch_then (qspecl_then [‘t1 with locals :=
+                                t.locals |+ (ctxt.max_var + 1,Word 0w)’, ‘0w’] mp_tac) >>
+      impl_tac
+      >- (
+       conj_tac
+       >- (
+        fs [word_0_n2w] >>
+        imp_res_tac locals_rel_lookup_ctxt >> rveq >>
+        fs [length_flatten_eq_size_of_shape] >> rfs []) >>
+       conj_tac
+       >- (
+        rw [] >>
+        ‘n <> ctxt.max_var + 1’ suffices_by (
+                                fs [FLOOKUP_UPDATE, locals_rel_def] >>
+                                first_x_assum drule_all >> strip_tac >> fs [] >> rveq >>
+                                imp_res_tac opt_mmap_mem_func >> fs []) >>
+        fs [locals_rel_def, ctxt_max_def] >>
+        last_x_assum drule_all >> strip_tac >> fs []) >>
+       rw [] >> rfs [] >>
+       drule locals_rel_lookup_ctxt >>
+       ‘size_of_shape (shape_of x) = LENGTH r''’ by (
+         drule locals_rel_lookup_ctxt >>
+         disch_then drule >>
+         strip_tac >> fs [] >> rveq >>
+         fs [length_flatten_eq_size_of_shape] >> rfs []) >>
+       fs [] >> drule opt_mmap_mem_func >>
+       disch_then drule >> strip_tac >> fs []) >>
+      strip_tac >> fs [] >>
+      conj_tac >- fs [state_rel_def] >>
+      conj_tac >- fs [Abbr ‘nctxt’, code_rel_def, ctxt_fc_code_vars_eq, ctxt_fc_eid_map_eq] >>
+      conj_tac
+      >- (
+       fs [Abbr ‘nctxt’, excp_rel_def, ctxt_fc_code_vars_eq, ctxt_fc_eid_map_eq]) >>
+      ‘MAP (λn. THE (FLOOKUP t1.globals n)) (GENLIST (λx. n2w x) (LENGTH r'')) =
+       flatten v’ by (
+        fs [opt_mmap_eq_some] >>
+        ‘size_of_shape (shape_of v) = LENGTH r''’ by (
+          drule locals_rel_lookup_ctxt >>
+          disch_then drule >>
+          strip_tac >> fs [] >> rveq >>
+          fs [length_flatten_eq_size_of_shape] >> rfs []) >>
+        fs [] >> drule map_some_the_map >> fs []) >>
+      fs [] >>
+      match_mp_tac local_rel_le_zip_update_preserved >> fs [] >>
+      match_mp_tac local_rel_gt_max_var_preserved >>
+      fs []
+
+val return_handle_tac =
+    (* Return case *)
     rename [‘FLOOKUP ctxt.var_nums rt’] >>
     TOP_CASE_TAC >> fs []
     (* eid_map = NONE case *)
@@ -5173,19 +5456,159 @@ Proof
     TOP_CASE_TAC >> fs []
     >- (
      TOP_CASE_TAC >> fs []
-     >- handle_ret_ret_case >>
+      >- handle_ret_ret_case >>
      TOP_CASE_TAC >> fs [] >>
      TOP_CASE_TAC >> fs []
      >- handle_ret_ret_case >>
-     TOP_CASE_TAC >> fs []
+     reverse TOP_CASE_TAC >> fs []
      >- handle_ret_ret_case >>
-     handle_ret_ret_case) >>
-    cheat (* when eid has comb shape *))
-   >- ((* Exception case *)
-    rename [‘FLOOKUP ctxt.var_nums rt’] >>
-    TOP_CASE_TAC >> fs []
-    (* eid_map = NONE case *)
-    >- (
+
+
+
+
+      rename [‘is_valid_value s.locals m v’] >>
+      fs [is_valid_value_def] >>
+      cases_on ‘FLOOKUP s.locals m’ >> fs [] >>
+      TOP_CASE_TAC >> fs []
+      >- (fs [locals_rel_def] >> first_x_assum drule >> fs []) >>
+      TOP_CASE_TAC >> fs [] >>
+      TOP_CASE_TAC >> fs []
+      >- (
+       TOP_CASE_TAC >> fs []
+       >- (
+        fs [locals_rel_def] >> first_x_assum drule >> fs [] >>
+        fs [OPT_MMAP_def] >>
+        strip_tac >> fs [] >>
+        pop_assum (assume_tac o GSYM) >>
+        ‘size_of_shape (shape_of x) = 1’ by
+          fs [panLangTheory.size_of_shape_def, shape_of_def] >>
+        fs [GSYM length_flatten_eq_size_of_shape] >> rfs [flatten_def]) >>
+       eval_call_impl_only_tac >>
+       strip_tac >> fs [] >>
+       ‘size_of_shape (shape_of x) = 1’ by (
+         fs [locals_rel_def] >>
+         last_x_assum drule >>
+         fs [shape_of_def]) >>
+       fs [shape_of_def] >>
+       fs [state_rel_def, panSemTheory.set_var_def,set_var_def,
+           Abbr ‘nctxt’, code_rel_def, ctxt_fc_code_vars_eq,ctxt_fc_eid_map_eq,
+           panSemTheory.set_var_def,set_var_def] >>
+       conj_tac
+       >- (
+        fs [excp_rel_def, ctxt_fc_code_vars_eq,ctxt_fc_eid_map_eq,
+            panSemTheory.set_var_def,set_var_def]) >>
+       ‘size_of_shape (shape_of v) = 1’ by fs [] >>
+       drule locals_rel_lookup_ctxt >>
+       disch_then drule >> strip_tac >> fs [] >>
+       rveq >> fs [length_flatten_eq_size_of_shape] >>
+       rfs [panLangTheory.size_of_shape_def] >>
+       fs [locals_rel_def, panSemTheory.set_var_def,set_var_def] >>
+       rw [] >> rveq >>
+       fs [FLOOKUP_UPDATE] >>
+       FULL_CASE_TAC >> fs [] >> rveq
+       >- (
+        fs [OPT_MMAP_def, FLOOKUP_UPDATE] >> rveq >>
+        fs [length_flatten_eq_size_of_shape, panLangTheory.size_of_shape_def]) >>
+       res_tac >> fs [] >>
+       match_mp_tac opt_mmap_flookup_update >>
+       fs [] >>
+       drule no_overlap_flookup_distinct >>
+       disch_then drule_all >> fs [distinct_lists_def]) >>
+      TOP_CASE_TAC >> fs []
+      >- (
+       ‘LENGTH r'' = 1’ by (
+         drule_all locals_rel_lookup_ctxt >> strip_tac >>
+         fs [length_flatten_eq_size_of_shape] >>
+         rfs [panLangTheory.size_of_shape_def]) >>
+       fs [] >>
+       cases_on ‘r''’ >> fs [ooHD_def] >>
+       eval_call_impl_only_tac >>
+       strip_tac >> fs [] >>
+       ‘size_of_shape (shape_of x) = 1’ by (
+         drule_all locals_rel_lookup_ctxt >> strip_tac >>
+         fs [length_flatten_eq_size_of_shape] >>
+         rfs [panLangTheory.size_of_shape_def]) >>
+       fs [shape_of_def, panLangTheory.size_of_shape_def] >>
+       fs [state_rel_def, panSemTheory.set_var_def,set_var_def,
+           Abbr ‘nctxt’, code_rel_def, ctxt_fc_code_vars_eq,ctxt_fc_eid_map_eq,
+           panSemTheory.set_var_def,set_var_def] >>
+       conj_tac
+       >- (
+        fs [excp_rel_def, ctxt_fc_code_vars_eq,ctxt_fc_eid_map_eq,
+            panSemTheory.set_var_def,set_var_def]) >>
+       ‘size_of_shape (shape_of v) = 1’ by fs [] >>
+       drule locals_rel_lookup_ctxt >>
+       disch_then drule >> strip_tac >> fs [] >>
+       rveq >> fs [length_flatten_eq_size_of_shape] >>
+       rfs [panLangTheory.size_of_shape_def] >>
+       fs [locals_rel_def, panSemTheory.set_var_def,set_var_def] >>
+       rw [] >> rveq >>
+       fs [FLOOKUP_UPDATE] >>
+       FULL_CASE_TAC >> fs [] >> rveq
+       >- (
+        fs [OPT_MMAP_def, FLOOKUP_UPDATE] >> rveq >>
+        fs [length_flatten_eq_size_of_shape, panLangTheory.size_of_shape_def]) >>
+       res_tac >> fs [] >>
+       match_mp_tac opt_mmap_flookup_update >>
+       fs [] >>
+       drule no_overlap_flookup_distinct >>
+       disch_then drule_all >> fs [distinct_lists_def]) >>
+
+
+
+      eval_call_append_code_impl_only_tac >>
+      fs [] >> strip_tac >>
+      ‘nctxt.eid_map = ctxt.eid_map’ by
+        fs [Abbr ‘nctxt’, ctxt_fc_eid_map_eq] >>
+      fs [shape_of_def, panLangTheory.size_of_shape_def,
+          panSemTheory.set_var_def, set_var_def] >>
+      cases_on ‘size_of_shape (shape_of x) = 0’ >> fs []
+      >- (
+       conj_tac >- fs [state_rel_def] >>
+       conj_tac >- fs [Abbr ‘nctxt’ , code_rel_def,
+                       ctxt_fc_code_vars_eq, ctxt_fc_eid_map_eq] >>
+       conj_tac
+       >- (
+        fs [Abbr ‘nctxt’, excp_rel_def,
+            ctxt_fc_code_vars_eq, ctxt_fc_eid_map_eq]) >>
+       ‘LENGTH (flatten v) = 0’ by (
+         rewrite_tac [length_flatten_eq_size_of_shape] >>
+         rfs []) >>
+       fs [locals_rel_def] >> rw [] >>
+       fs [FLOOKUP_UPDATE] >> FULL_CASE_TAC >> fs [] >> rveq
+       >- ( cheat (* annoying cheat *) (*
+        fs [OPT_MMAP_def] >>
+        ‘LENGTH (flatten x) = 0’ suffices_by fs[] >>
+        rewrite_tac [length_flatten_eq_size_of_shape] >>
+        fs [] *)) >>
+       first_x_assum drule >> strip_tac >> fs [] >>
+       fs [opt_mmap_eq_some, MAP_EQ_EVERY2, LIST_REL_EL_EQN] >>
+       rw [] >> fs [FLOOKUP_UPDATE] >>
+       TOP_CASE_TAC >> fs [] >>
+       drule ctxt_max_el_leq >>
+       qpat_x_assum ‘LENGTH _ = LENGTH (flatten _)’ (assume_tac o GSYM) >>
+       fs [] >> disch_then drule_all >> fs []) >>
+      ‘1 < size_of_shape (shape_of x)’ by (
+        drule locals_rel_lookup_ctxt >>
+        disch_then drule >>
+        strip_tac >> fs [] >> rfs [] >>
+        fs [panLangTheory.size_of_shape_def] >>
+        DECIDE_TAC) >>
+      ‘1 < size_of_shape (shape_of x)’ by cheat >> fs [] >>
+      conj_tac >- fs [state_rel_def] >>
+      conj_tac >- fs [Abbr ‘nctxt’ , code_rel_def,
+                      ctxt_fc_code_vars_eq, ctxt_fc_eid_map_eq] >>
+      conj_tac
+      >- (
+       fs [Abbr ‘nctxt’, excp_rel_def,
+           ctxt_fc_code_vars_eq, ctxt_fc_eid_map_eq]) >>
+      fs [locals_rel_def] >> rw [] >>
+      fs [FLOOKUP_UPDATE] >> FULL_CASE_TAC >> fs [] >> rveq >>
+      cheat) >>
+    cheat (* when eid has comb shape *)
+
+
+val excp_eid_none_handler_tac = (* eid_map = NONE case *)
      cases_on ‘m' = eid’ >> fs [] >> rveq >> rfs []
      >- (
       reverse (cases_on ‘FLOOKUP s.eshapes eid’) >> fs [] >>
@@ -5254,9 +5677,6 @@ Proof
         fs [Abbr ‘nctxt’, ctxt_fc_eid_map_eq] >>
       fs [] >>
       cases_on ‘x’ >> fs [] >>
-      ‘~MEM (uassigned_eid ctxt.eid_map) t.eids’ by (
-        fs [excp_rel_def] >> fs [uassigned_eid_def, shape_of_def, panLangTheory.size_of_shape_def]  >>
-        CCONTR_TAC >> fs [] >> fs [max_set_list_max, list_max_add_not_mem]) >>
       cases_on ‘size_of_shape (shape_of v) = 0’ >> fs []
       >- rels_empty_tac >>
       cases_on ‘size_of_shape (shape_of v) = 1’ >> fs []
@@ -5274,9 +5694,6 @@ Proof
         fs [Abbr ‘nctxt’, ctxt_fc_eid_map_eq] >>
       fs [] >>
       cases_on ‘x’ >> fs [] >>
-      ‘~MEM (uassigned_eid ctxt.eid_map) t.eids’ by (
-        fs [excp_rel_def] >> fs [uassigned_eid_def, shape_of_def, panLangTheory.size_of_shape_def]  >>
-        CCONTR_TAC >> fs [] >> fs [max_set_list_max, list_max_add_not_mem]) >>
       cases_on ‘size_of_shape (shape_of v) = 0’ >> fs []
       >- rels_empty_tac >>
       cases_on ‘size_of_shape (shape_of v) = 1’ >> fs []
@@ -5286,9 +5703,6 @@ Proof
       rels_empty_tac) >>
      eval_call_nested_seq_impl_only_tac >>
      strip_tac >> fs [] >>
-     ‘~MEM (uassigned_eid ctxt.eid_map) t.eids’ by (
-       fs [excp_rel_def] >> fs [uassigned_eid_def, shape_of_def, panLangTheory.size_of_shape_def]  >>
-       CCONTR_TAC >> fs [] >> fs [max_set_list_max, list_max_add_not_mem]) >>
      cases_on ‘res1’ >> fs [] >> rveq >> fs [] >>
      TRY (cases_on ‘x’ >> fs [] >> rveq >> fs []) >>
      cases_on ‘FLOOKUP ctxt.eid_map m'’ >> fs []
@@ -5303,692 +5717,303 @@ Proof
      >- (
       fs [shape_of_def, panLangTheory.size_of_shape_def] >>
       rels_empty_tac) >>
-     rels_empty_tac) >>
-    (* eid_map = SOME case *)
-    >- (
-     cases_on ‘m' = eid’ >> fs [] >> rveq >> rfs []
-     >- (
-      cases_on ‘FLOOKUP s.eshapes eid’ >> fs []
+     rels_empty_tac
+
+val handle_eid_one_evar_none =
+     (* evar = NONE case *)
+      cases_on ‘is_valid_value s.locals evar v’
       >- (
+       fs [is_valid_value_def] >>
+       cases_on ‘FLOOKUP s.locals evar’ >> fs [] >>
+       fs [locals_rel_def] >> res_tac >> fs []) >>
+      fs [] >> rveq >> fs [] >>
+      cases_on ‘m' = eid’ >> fs [] >> rveq >> fs []
+      >- (
+       TOP_CASE_TAC >> fs []
+       >- (
+        eval_call_impl_only_tac >>
+        strip_tac >> fs [] >>
+        ‘nctxt.eid_map = ctxt.eid_map’ by
+          fs [Abbr ‘nctxt’, ctxt_fc_eid_map_eq] >>
+        fs [] >>
+        cases_on ‘FLOOKUP ctxt.eid_map eid’ >> fs [] >>
+        cases_on ‘x’ >> fs [] >>
+        cases_on ‘size_of_shape (shape_of v) = 0’ >> fs []
+        >- rels_empty_tac >>
+        cases_on ‘size_of_shape (shape_of v) = 1’ >> fs []
+        >- (fs [shape_of_def, panLangTheory.size_of_shape_def] >> rels_empty_tac) >>
+        rels_empty_tac) >>
        TOP_CASE_TAC >> fs [] >>
        TOP_CASE_TAC >> fs []
        >- (
-        rename [‘FLOOKUP ctxt.var_nums evar’] >>
-        TOP_CASE_TAC >> fs []
-        >- ( (* evar = NONE case *)
-         TOP_CASE_TAC >> fs []
-         >- (
-          eval_call_impl_only_tac >>
-          strip_tac >> fs [] >>
-          ‘nctxt.eid_map = ctxt.eid_map’ by
-            fs [Abbr ‘nctxt’, ctxt_fc_eid_map_eq] >>
-          fs [] >>
-          cases_on ‘FLOOKUP ctxt.eid_map eid’ >> fs [] >>
-          cases_on ‘x’ >> fs [] >>
-          cases_on ‘size_of_shape (shape_of v) = 0’ >> fs []
-          >- rels_empty_tac >>
-          cases_on ‘size_of_shape (shape_of v) = 1’ >> fs []
-          >- (fs [shape_of_def, panLangTheory.size_of_shape_def] >> rels_empty_tac) >>
-          rels_empty_tac) >>
-         TOP_CASE_TAC >> fs [] >>
-         TOP_CASE_TAC >> fs []
-         >- (
-          TOP_CASE_TAC >> fs []
-          >- (
-           eval_call_impl_only_tac >>
-           strip_tac >> fs [] >>
-           ‘nctxt.eid_map = ctxt.eid_map’ by
-             fs [Abbr ‘nctxt’, ctxt_fc_eid_map_eq] >>
-           fs [] >>
-           cases_on ‘FLOOKUP ctxt.eid_map eid’ >> fs [] >>
-           cases_on ‘x’ >> fs [] >>
-           cases_on ‘size_of_shape (shape_of v) = 0’ >> fs []
-           >- rels_empty_tac >>
-           cases_on ‘size_of_shape (shape_of v) = 1’ >> fs []
-           >- (fs [shape_of_def, panLangTheory.size_of_shape_def] >> rels_empty_tac) >>
-           rels_empty_tac) >>
-          eval_call_impl_only_tac >>
-          strip_tac >> fs [] >>
-          ‘nctxt.eid_map = ctxt.eid_map’ by
-            fs [Abbr ‘nctxt’, ctxt_fc_eid_map_eq] >>
-           fs [] >>
-           cases_on ‘FLOOKUP ctxt.eid_map eid’ >> fs [] >>
-           ‘~MEM (uassigned_eid ctxt.eid_map) t.eids’ by (
-             fs [excp_rel_def] >> fs [uassigned_eid_def, shape_of_def, panLangTheory.size_of_shape_def]  >>
-             CCONTR_TAC >> fs [] >> fs [max_set_list_max, list_max_add_not_mem]) >> fs [] >>
-           cases_on ‘x’ >> fs [] >>
-           cases_on ‘size_of_shape (shape_of v) = 0’ >> fs []
-           >- rels_empty_tac >>
-           cases_on ‘size_of_shape (shape_of v) = 1’ >> fs []
-           >- (fs [shape_of_def, panLangTheory.size_of_shape_def] >> rels_empty_tac) >>
-           rels_empty_tac) >>
-         TOP_CASE_TAC >> fs [] >> rveq >> fs []
-         >- (
-          eval_call_impl_only_tac >>
-          strip_tac >> fs [] >>
-          ‘nctxt.eid_map = ctxt.eid_map’ by
-            fs [Abbr ‘nctxt’, ctxt_fc_eid_map_eq] >>
-          fs [] >>
-          cases_on ‘FLOOKUP ctxt.eid_map eid’ >> fs [] >>
-          ‘~MEM (uassigned_eid ctxt.eid_map) t.eids’ by (
-            fs [excp_rel_def] >> fs [uassigned_eid_def, shape_of_def, panLangTheory.size_of_shape_def]  >>
-            CCONTR_TAC >> fs [] >> fs [max_set_list_max, list_max_add_not_mem]) >> fs [] >>
-          cases_on ‘x’ >> fs [] >>
-          cases_on ‘size_of_shape (shape_of v) = 0’ >> fs []
-          >- rels_empty_tac >>
-          cases_on ‘size_of_shape (shape_of v) = 1’ >> fs []
-          >- (fs [shape_of_def, panLangTheory.size_of_shape_def] >> rels_empty_tac) >>
-          rels_empty_tac) >>
-         eval_call_nested_seq_impl_only_tac >>
-         strip_tac >> fs [] >>
-         ‘nctxt.eid_map = ctxt.eid_map’ by
-           fs [Abbr ‘nctxt’, ctxt_fc_eid_map_eq] >>
-         fs [] >>
-         ‘~MEM (uassigned_eid ctxt.eid_map) t.eids’ by (
-           fs [excp_rel_def] >> fs [uassigned_eid_def, shape_of_def, panLangTheory.size_of_shape_def]  >>
-           CCONTR_TAC >> fs [] >> fs [max_set_list_max, list_max_add_not_mem]) >> fs [] >>
-         cases_on ‘res1’ >> fs [] >> rveq >> fs [] >>
-         TRY (cases_on ‘x’ >> fs [] >> rveq >> fs []) >>
-         cases_on ‘FLOOKUP ctxt.eid_map eid’ >> fs [] >>
-         cases_on ‘x’ >> fs [] >>
-         rveq >> fs [] >>
-         cases_on ‘size_of_shape (shape_of v) = 0’ >> fs []
-         >- rels_empty_tac >>
-         cases_on ‘size_of_shape (shape_of v) = 1’ >> fs []
-         >- (
-          fs [shape_of_def, panLangTheory.size_of_shape_def] >>
-          rels_empty_tac) >>
-         rels_empty_tac) >>
-        TOP_CASE_TAC >> fs [] >>
         TOP_CASE_TAC >> fs []
         >- (
-         TOP_CASE_TAC >> fs []
-         >- (
-          eval_call_impl_only_tac >>
-          strip_tac >> fs [] >>
-          ‘nctxt.eid_map = ctxt.eid_map’ by
-            fs [Abbr ‘nctxt’, ctxt_fc_eid_map_eq] >>
-          fs [] >>
-          cases_on ‘FLOOKUP ctxt.eid_map eid’ >> fs [] >>
-          cases_on ‘x’ >> fs [] >>
-          cases_on ‘size_of_shape (shape_of v) = 0’ >> fs []
-          >- rels_empty_tac >>
-          cases_on ‘size_of_shape (shape_of v) = 1’ >> fs []
-          >- (fs [shape_of_def, panLangTheory.size_of_shape_def] >> rels_empty_tac) >>
-          rels_empty_tac) >>
-         TOP_CASE_TAC >> fs [] >>
-         TOP_CASE_TAC >> fs [] >> rveq >> fs []
-         >- (
-          TOP_CASE_TAC >> fs []
-          >- (
-           eval_call_impl_only_tac >>
-           strip_tac >> fs [] >>
-           ‘nctxt.eid_map = ctxt.eid_map’ by
-             fs [Abbr ‘nctxt’, ctxt_fc_eid_map_eq] >>
-           fs [] >>
-           cases_on ‘FLOOKUP ctxt.eid_map eid’ >> fs [] >>
-           cases_on ‘x’ >> fs [] >>
-           cases_on ‘size_of_shape (shape_of v) = 0’ >> fs []
-           >- rels_empty_tac >>
-           cases_on ‘size_of_shape (shape_of v) = 1’ >> fs []
-           >- (fs [shape_of_def, panLangTheory.size_of_shape_def] >> rels_empty_tac) >>
-           rels_empty_tac) >>
-          eval_call_impl_only_tac >>
-          strip_tac >> fs [] >>
-          ‘nctxt.eid_map = ctxt.eid_map’ by
-            fs [Abbr ‘nctxt’, ctxt_fc_eid_map_eq] >>
-           fs [] >>
-           cases_on ‘FLOOKUP ctxt.eid_map eid’ >> fs [] >>
-           ‘~MEM (uassigned_eid ctxt.eid_map) t.eids’ by (
-             fs [excp_rel_def] >> fs [uassigned_eid_def, shape_of_def, panLangTheory.size_of_shape_def]  >>
-             CCONTR_TAC >> fs [] >> fs [max_set_list_max, list_max_add_not_mem]) >> fs [] >>
-           cases_on ‘x’ >> fs [] >>
-           cases_on ‘size_of_shape (shape_of v) = 0’ >> fs []
-           >- rels_empty_tac >>
-           cases_on ‘size_of_shape (shape_of v) = 1’ >> fs []
-           >- (fs [shape_of_def, panLangTheory.size_of_shape_def] >> rels_empty_tac) >>
-           rels_empty_tac) >>
-         TOP_CASE_TAC >> fs [] >> rveq >> fs []
-         >- (
-          eval_call_impl_only_tac >>
-          strip_tac >> fs [] >>
-          ‘nctxt.eid_map = ctxt.eid_map’ by
-            fs [Abbr ‘nctxt’, ctxt_fc_eid_map_eq] >>
-           fs [] >>
-           cases_on ‘FLOOKUP ctxt.eid_map eid’ >> fs [] >>
-           ‘~MEM (uassigned_eid ctxt.eid_map) t.eids’ by (
-             fs [excp_rel_def] >> fs [uassigned_eid_def, shape_of_def, panLangTheory.size_of_shape_def]  >>
-             CCONTR_TAC >> fs [] >> fs [max_set_list_max, list_max_add_not_mem]) >> fs [] >>
-           cases_on ‘x’ >> fs [] >>
-           cases_on ‘size_of_shape (shape_of v) = 0’ >> fs []
-           >- rels_empty_tac >>
-           cases_on ‘size_of_shape (shape_of v) = 1’ >> fs []
-           >- (fs [shape_of_def, panLangTheory.size_of_shape_def] >> rels_empty_tac) >>
-           rels_empty_tac) >>
-         eval_call_nested_seq_impl_only_tac >>
-         strip_tac >> fs [] >>
-         ‘nctxt.eid_map = ctxt.eid_map’ by
-           fs [Abbr ‘nctxt’, ctxt_fc_eid_map_eq] >>
-         fs [] >>
-         ‘~MEM (uassigned_eid ctxt.eid_map) t.eids’ by (
-           fs [excp_rel_def] >> fs [uassigned_eid_def, shape_of_def, panLangTheory.size_of_shape_def]  >>
-           CCONTR_TAC >> fs [] >> fs [max_set_list_max, list_max_add_not_mem]) >> fs [] >>
-         cases_on ‘res1’ >> fs [] >> rveq >> fs [] >>
-         TRY (cases_on ‘x’ >> fs [] >> rveq >> fs []) >>
-         cases_on ‘FLOOKUP ctxt.eid_map eid’ >> fs [] >>
-         cases_on ‘x’ >> fs [] >>
-         rveq >> fs [] >>
-         cases_on ‘size_of_shape (shape_of v) = 0’ >> fs []
-         >- rels_empty_tac >>
-         cases_on ‘size_of_shape (shape_of v) = 1’ >> fs []
-         >- (
-          fs [shape_of_def, panLangTheory.size_of_shape_def] >>
-          rels_empty_tac) >>
-         rels_empty_tac) >>
-        TOP_CASE_TAC >> fs [] >> rveq >> fs []
-        >- (
-         TOP_CASE_TAC >> fs []
-         >- (
-          eval_call_impl_only_tac >>
-          strip_tac >> fs [] >>
-          ‘nctxt.eid_map = ctxt.eid_map’ by
-            fs [Abbr ‘nctxt’, ctxt_fc_eid_map_eq] >>
-          fs [] >>
-          cases_on ‘FLOOKUP ctxt.eid_map eid’ >> fs [] >>
-          cases_on ‘x’ >> fs [] >>
-          cases_on ‘size_of_shape (shape_of v) = 0’ >> fs []
-          >- rels_empty_tac >>
-          cases_on ‘size_of_shape (shape_of v) = 1’ >> fs []
-          >- (fs [shape_of_def, panLangTheory.size_of_shape_def] >> rels_empty_tac) >>
-          rels_empty_tac) >>
-         TOP_CASE_TAC >> fs [] >>
-         TOP_CASE_TAC >> fs []
-         >- (
-          TOP_CASE_TAC >> fs []
-          >- (
-          eval_call_impl_only_tac >>
-          strip_tac >> fs [] >>
-          ‘nctxt.eid_map = ctxt.eid_map’ by
-            fs [Abbr ‘nctxt’, ctxt_fc_eid_map_eq] >>
-          fs [] >>
-          cases_on ‘FLOOKUP ctxt.eid_map eid’ >> fs [] >>
-          cases_on ‘x’ >> fs [] >>
-          cases_on ‘size_of_shape (shape_of v) = 0’ >> fs []
-          >- rels_empty_tac >>
-          cases_on ‘size_of_shape (shape_of v) = 1’ >> fs []
-          >- (fs [shape_of_def, panLangTheory.size_of_shape_def] >> rels_empty_tac) >>
-          rels_empty_tac) >>
          eval_call_impl_only_tac >>
          strip_tac >> fs [] >>
          ‘nctxt.eid_map = ctxt.eid_map’ by
            fs [Abbr ‘nctxt’, ctxt_fc_eid_map_eq] >>
          fs [] >>
          cases_on ‘FLOOKUP ctxt.eid_map eid’ >> fs [] >>
-         cases_on ‘x’ >> fs [] >> rveq >> fs [] >>
-         ‘MEM r' t.eids’ by cheat >>
-         cases_on ‘size_of_shape (shape_of v) = 0’ >> fs []
-          >- rels_empty_tac >>
-
-
-
-
-           )
-
-
-
-          )
-
-
-         )
-
-
-
-
-
-
-
-         TOP_CASE_TAC >> fs [] >>
-         TOP_CASE_TAC >> fs []
-         >- (
-          TOP_CASE_TAC >> fs []
-          >- (
-           eval_call_impl_only_tac >>
-           strip_tac >> fs [] >>
-           ‘nctxt.eid_map = ctxt.eid_map’ by
-             fs [Abbr ‘nctxt’, ctxt_fc_eid_map_eq] >>
-           fs [] >>
-           cases_on ‘FLOOKUP ctxt.eid_map eid’ >> fs [] >>
-           cases_on ‘x’ >> fs [] >>
-           cases_on ‘size_of_shape (shape_of v) = 0’ >> fs []
-           >- rels_empty_tac >>
-           cases_on ‘size_of_shape (shape_of v) = 1’ >> fs []
-           >- (fs [shape_of_def, panLangTheory.size_of_shape_def] >> rels_empty_tac) >>
-           rels_empty_tac) >>
-          eval_call_impl_only_tac >>
-          strip_tac >> fs [] >>
-          ‘nctxt.eid_map = ctxt.eid_map’ by
-            fs [Abbr ‘nctxt’, ctxt_fc_eid_map_eq] >>
-           fs [] >>
-           cases_on ‘FLOOKUP ctxt.eid_map eid’ >> fs [] >>
-           ‘~MEM (uassigned_eid ctxt.eid_map) t.eids’ by (
-             fs [excp_rel_def] >> fs [uassigned_eid_def, shape_of_def, panLangTheory.size_of_shape_def]  >>
-             CCONTR_TAC >> fs [] >> fs [max_set_list_max, list_max_add_not_mem]) >> fs [] >>
-           cases_on ‘x’ >> fs [] >>
-           cases_on ‘size_of_shape (shape_of v) = 0’ >> fs []
-           >- rels_empty_tac >>
-           cases_on ‘size_of_shape (shape_of v) = 1’ >> fs []
-           >- (fs [shape_of_def, panLangTheory.size_of_shape_def] >> rels_empty_tac) >>
-           rels_empty_tac) >>
-         TOP_CASE_TAC >> fs [] >> rveq >> fs []
-         >- (
-          eval_call_impl_only_tac >>
-          strip_tac >> fs [] >>
-          ‘nctxt.eid_map = ctxt.eid_map’ by
-            fs [Abbr ‘nctxt’, ctxt_fc_eid_map_eq] >>
-          fs [] >>
-          cases_on ‘FLOOKUP ctxt.eid_map eid’ >> fs [] >>
-          ‘~MEM (uassigned_eid ctxt.eid_map) t.eids’ by (
-            fs [excp_rel_def] >> fs [uassigned_eid_def, shape_of_def, panLangTheory.size_of_shape_def]  >>
-            CCONTR_TAC >> fs [] >> fs [max_set_list_max, list_max_add_not_mem]) >> fs [] >>
-          cases_on ‘x’ >> fs [] >>
-          cases_on ‘size_of_shape (shape_of v) = 0’ >> fs []
-          >- rels_empty_tac >>
-          cases_on ‘size_of_shape (shape_of v) = 1’ >> fs []
-          >- (fs [shape_of_def, panLangTheory.size_of_shape_def] >> rels_empty_tac) >>
-          rels_empty_tac) >>
-         eval_call_nested_seq_impl_only_tac >>
-         strip_tac >> fs [] >>
-         ‘nctxt.eid_map = ctxt.eid_map’ by
-           fs [Abbr ‘nctxt’, ctxt_fc_eid_map_eq] >>
-         fs [] >>
-         ‘~MEM (uassigned_eid ctxt.eid_map) t.eids’ by (
-           fs [excp_rel_def] >> fs [uassigned_eid_def, shape_of_def, panLangTheory.size_of_shape_def]  >>
-           CCONTR_TAC >> fs [] >> fs [max_set_list_max, list_max_add_not_mem]) >> fs [] >>
-         cases_on ‘res1’ >> fs [] >> rveq >> fs [] >>
-         TRY (cases_on ‘x’ >> fs [] >> rveq >> fs []) >>
-         cases_on ‘FLOOKUP ctxt.eid_map eid’ >> fs [] >>
          cases_on ‘x’ >> fs [] >>
-         rveq >> fs [] >>
          cases_on ‘size_of_shape (shape_of v) = 0’ >> fs []
          >- rels_empty_tac >>
          cases_on ‘size_of_shape (shape_of v) = 1’ >> fs []
-         >- (
-          fs [shape_of_def, panLangTheory.size_of_shape_def] >>
-          rels_empty_tac) >>
+         >- (fs [shape_of_def, panLangTheory.size_of_shape_def] >> rels_empty_tac) >>
          rels_empty_tac) >>
-        TOP_CASE_TAC >> fs [] >> rveq >> fs []
-        >- cheat >>
-        cheat
-
-
-
-
-
-
-
-
-                (
-         TOP_CASE_TAC >> fs []
-         >- (
-          eval_call_impl_only_tac >>
-          strip_tac >> fs [] >>
-          ‘nctxt.eid_map = ctxt.eid_map’ by
-            fs [Abbr ‘nctxt’, ctxt_fc_eid_map_eq] >>
-          fs [] >>
-          cases_on ‘FLOOKUP ctxt.eid_map eid’ >> fs [] >>
-          cases_on ‘x’ >> fs [] >>
-          cases_on ‘size_of_shape (shape_of v) = 0’ >> fs []
-          >- rels_empty_tac >>
-          cases_on ‘size_of_shape (shape_of v) = 1’ >> fs []
-          >- (fs [shape_of_def, panLangTheory.size_of_shape_def] >> rels_empty_tac) >>
-          rels_empty_tac) >>
-         TOP_CASE_TAC >> fs []
-         >- (
-          eval_call_impl_only_tac >>
-          strip_tac >> fs [] >>
-          ‘nctxt.eid_map = ctxt.eid_map’ by
-            fs [Abbr ‘nctxt’, ctxt_fc_eid_map_eq] >>
-          fs [] >>
-          cases_on ‘FLOOKUP ctxt.eid_map eid’ >> fs [] >>
-          cases_on ‘x’ >> fs [] >>
-          cases_on ‘size_of_shape (shape_of v) = 0’ >> fs []
-          >- rels_empty_tac >>
-          cases_on ‘size_of_shape (shape_of v) = 1’ >> fs []
-          >- (fs [shape_of_def, panLangTheory.size_of_shape_def] >> rels_empty_tac) >>
-          rels_empty_tac) >>
-         TOP_CASE_TAC >> fs [] >>
-         TOP_CASE_TAC >> fs []
-         >- (
-          TOP_CASE_TAC >> fs []
-          >- (
-           eval_call_impl_only_tac >>
-           strip_tac >> fs [] >>
-           ‘nctxt.eid_map = ctxt.eid_map’ by
-             fs [Abbr ‘nctxt’, ctxt_fc_eid_map_eq] >>
-           fs [] >>
-           cases_on ‘FLOOKUP ctxt.eid_map eid’ >> fs [] >>
-           cases_on ‘x’ >> fs [] >>
-           cases_on ‘size_of_shape (shape_of v) = 0’ >> fs []
-           >- rels_empty_tac >>
-           cases_on ‘size_of_shape (shape_of v) = 1’ >> fs []
-           >- (fs [shape_of_def, panLangTheory.size_of_shape_def] >> rels_empty_tac) >>
-           rels_empty_tac) >>
-          eval_call_impl_only_tac >>
-          strip_tac >> fs [] >>
-          ‘nctxt.eid_map = ctxt.eid_map’ by
-            fs [Abbr ‘nctxt’, ctxt_fc_eid_map_eq] >>
-           fs [] >>
-           cases_on ‘FLOOKUP ctxt.eid_map eid’ >> fs [] >>
-           ‘~MEM (uassigned_eid ctxt.eid_map) t.eids’ by (
-             fs [excp_rel_def] >> fs [uassigned_eid_def, shape_of_def, panLangTheory.size_of_shape_def]  >>
-             CCONTR_TAC >> fs [] >> fs [max_set_list_max, list_max_add_not_mem]) >> fs [] >>
-           cases_on ‘x’ >> fs [] >>
-           cases_on ‘size_of_shape (shape_of v) = 0’ >> fs []
-           >- rels_empty_tac >>
-           cases_on ‘size_of_shape (shape_of v) = 1’ >> fs []
-           >- (fs [shape_of_def, panLangTheory.size_of_shape_def] >> rels_empty_tac) >>
-           rels_empty_tac) >>
-         TOP_CASE_TAC >> fs [] >> rveq >> fs []
-         >- (
-          eval_call_impl_only_tac >>
-          strip_tac >> fs [] >>
-          ‘nctxt.eid_map = ctxt.eid_map’ by
-            fs [Abbr ‘nctxt’, ctxt_fc_eid_map_eq] >>
-          fs [] >>
-          cases_on ‘FLOOKUP ctxt.eid_map eid’ >> fs [] >>
-          ‘~MEM (uassigned_eid ctxt.eid_map) t.eids’ by (
-            fs [excp_rel_def] >> fs [uassigned_eid_def, shape_of_def, panLangTheory.size_of_shape_def]  >>
-            CCONTR_TAC >> fs [] >> fs [max_set_list_max, list_max_add_not_mem]) >> fs [] >>
-          cases_on ‘x’ >> fs [] >>
-          cases_on ‘size_of_shape (shape_of v) = 0’ >> fs []
-          >- rels_empty_tac >>
-          cases_on ‘size_of_shape (shape_of v) = 1’ >> fs []
-          >- (fs [shape_of_def, panLangTheory.size_of_shape_def] >> rels_empty_tac) >>
-          rels_empty_tac) >>
-         eval_call_nested_seq_impl_only_tac >>
-         strip_tac >> fs [] >>
-         ‘nctxt.eid_map = ctxt.eid_map’ by
-           fs [Abbr ‘nctxt’, ctxt_fc_eid_map_eq] >>
-         fs [] >>
-         ‘~MEM (uassigned_eid ctxt.eid_map) t.eids’ by (
-           fs [excp_rel_def] >> fs [uassigned_eid_def, shape_of_def, panLangTheory.size_of_shape_def]  >>
-           CCONTR_TAC >> fs [] >> fs [max_set_list_max, list_max_add_not_mem]) >> fs [] >>
-         cases_on ‘res1’ >> fs [] >> rveq >> fs [] >>
-         TRY (cases_on ‘x’ >> fs [] >> rveq >> fs []) >>
-         cases_on ‘FLOOKUP ctxt.eid_map eid’ >> fs [] >>
-         cases_on ‘x’ >> fs [] >>
-         rveq >> fs [] >>
-         cases_on ‘size_of_shape (shape_of v) = 0’ >> fs []
-         >- rels_empty_tac >>
-         cases_on ‘size_of_shape (shape_of v) = 1’ >> fs []
-         >- (
-          fs [shape_of_def, panLangTheory.size_of_shape_def] >>
-          rels_empty_tac) >>
-         rels_empty_tac)
-
-
-
-
-         eval_call_impl_only_tac >>
-         strip_tac >> fs [] >>
-          ‘nctxt.eid_map = ctxt.eid_map’ by
-            fs [Abbr ‘nctxt’, ctxt_fc_eid_map_eq] >>
-           fs [] >>
-           cases_on ‘FLOOKUP ctxt.eid_map eid’ >> fs [] >>
-           ‘~MEM (uassigned_eid ctxt.eid_map) t.eids’ by (
-             fs [excp_rel_def] >> fs [uassigned_eid_def, shape_of_def, panLangTheory.size_of_shape_def]  >>
-             CCONTR_TAC >> fs [] >> fs [max_set_list_max, list_max_add_not_mem]) >> fs [] >>
-           cases_on ‘x’ >> fs [] >>
-           cases_on ‘size_of_shape (shape_of v) = 0’ >> fs []
-           >- rels_empty_tac >>
-           cases_on ‘size_of_shape (shape_of v) = 1’ >> fs []
-           >- (fs [shape_of_def, panLangTheory.size_of_shape_def] >> rels_empty_tac) >>
-           rels_empty_tac)
-
-
-
-         )
-
-
-
-
-
-
-
-
-
-
-
-
-
-
-
-
-
-
-
-         ‘~MEM (uassigned_eid ctxt.eid_map) t.eids’ by (
-           fs [excp_rel_def] >> fs [uassigned_eid_def, shape_of_def, panLangTheory.size_of_shape_def]  >>
-           CCONTR_TAC >> fs [] >> fs [max_set_list_max, list_max_add_not_mem]) >>
-         cases_on ‘res1’ >> fs [] >> rveq >> fs [] >>
-         TRY (cases_on ‘x’ >> fs [] >> rveq >> fs []) >>
-         cases_on ‘FLOOKUP ctxt.eid_map eid’ >> fs []
-         >- fs [Abbr ‘nctxt’, ctxt_fc_eid_map_eq] >>
-         ‘nctxt.eid_map = ctxt.eid_map’ by
-           fs [Abbr ‘nctxt’, ctxt_fc_eid_map_eq] >>
-         fs [] >>
-         cases_on ‘x’ >> fs [] >>
-         cases_on ‘size_of_shape (shape_of v) = 0’ >> fs []
-         >- rels_empty_tac >>
-         cases_on ‘size_of_shape (shape_of v) = 1’ >> fs []
-         >- (
-          fs [shape_of_def, panLangTheory.size_of_shape_def] >>
-          rels_empty_tac) >>
-         rels_empty_tac)
-
-
-
-
-          )
-
-
-
-
-
-
-
-
-
-
-
-
-
-
-
-
-
-
-
-
-
-
-
-          )
-
-
-         )
-
-        )
-
-
-       )
-      rveq >> fs []
-      >- (fs [excp_rel_def] >> res_tac >> rfs []) >>
-      >-
-
-
-      cases_on ‘x’ >> fs [] >>
-      cases_on ‘q’ >> fs []
-      >- ((* lookup eid = SOME (One, _) *)
-       reverse (cases_on ‘FLOOKUP s.eshapes eid’) >> fs [] >>
-       rveq >> fs []
-       >- (fs [excp_rel_def] >> res_tac >> fs []) >>
-       rename [‘FLOOKUP ctxt.var_nums evar’]
-
-
-       )
-
-
-
-
-      reverse (cases_on ‘FLOOKUP s.eshapes eid’) >> fs [] >>
-      rveq >> fs []
-      >- (fs [excp_rel_def] >> res_tac >> fs []) >>
-      fs [panSemTheory.lookup_code_def, CaseEq "option", CaseEq "prod"] >> rveq >>
-      drule code_rel_imp >>
-      disch_then drule >>
-      strip_tac >> fs [] >>
-      fs [lookup_code_def] >>
-      drule (INST_TYPE [``:'c``|->``:num``] list_rel_length_shape_of_flatten) >>
-      disch_then (qspec_then ‘ns’ mp_tac) >>
-      fs [] >>
-      strip_tac >>
-      qmatch_asmsub_abbrev_tac ‘compile_prog nctxt _’ >>
-      first_x_assum (qspecl_then
-                     [‘dec_clock t with
-                       locals := FEMPTY |++ ZIP (ns,FLAT (MAP flatten args))’,
-                      ‘nctxt’] mp_tac) >>
-      impl_tac
-      >- (
-       fs [Abbr ‘nctxt’, slc_tlc_rw] >>
-       match_mp_tac call_preserve_state_code_locals_rel >>
-       fs []) >>
-      strip_tac >> fs [] >>
-      rfs [Abbr ‘nctxt’, ctxt_fc_eid_map_eq]) >>
-     TOP_CASE_TAC >> fs []
-     >- (
-      eval_call_impl_only_tac >>
-      strip_tac >> fs [] >>
-      cases_on ‘FLOOKUP ctxt.eid_map m'’ >> fs []
-      >- fs [Abbr ‘nctxt’, ctxt_fc_eid_map_eq] >>
-      ‘nctxt.eid_map = ctxt.eid_map’ by
-        fs [Abbr ‘nctxt’, ctxt_fc_eid_map_eq] >>
-      fs [] >>
-      cases_on ‘x’ >> fs [] >>
-      cases_on ‘size_of_shape (shape_of v) = 0’ >> fs []
-     >- rels_empty_tac >>
-     cases_on ‘size_of_shape (shape_of v) = 1’ >> fs []
-     >- (fs [shape_of_def, panLangTheory.size_of_shape_def] >> rels_empty_tac) >>
-     rels_empty_tac) >>
-     TOP_CASE_TAC >> fs [] >>
-     TOP_CASE_TAC >> fs []
-     >- (
+        eval_call_impl_only_tac >>
+        strip_tac >> fs [] >>
+        ‘nctxt.eid_map = ctxt.eid_map’ by
+          fs [Abbr ‘nctxt’, ctxt_fc_eid_map_eq] >>
+        fs [] >>
+        cases_on ‘FLOOKUP ctxt.eid_map eid’ >> fs [] >>
+        cases_on ‘x’ >> fs [] >>
+        cases_on ‘size_of_shape (shape_of v) = 0’ >> fs []
+        >- rels_empty_tac >>
+        cases_on ‘size_of_shape (shape_of v) = 1’ >> fs []
+        >- (fs [shape_of_def, panLangTheory.size_of_shape_def] >> rels_empty_tac) >>
+        rels_empty_tac) >>
+       TOP_CASE_TAC >> fs [] >> rveq >> fs []
+       >- (
+        eval_call_impl_only_tac >>
+        strip_tac >> fs [] >>
+        ‘nctxt.eid_map = ctxt.eid_map’ by
+          fs [Abbr ‘nctxt’, ctxt_fc_eid_map_eq] >>
+        fs [] >>
+        cases_on ‘FLOOKUP ctxt.eid_map eid’ >> fs [] >>
+        cases_on ‘x’ >> fs [] >>
+        cases_on ‘size_of_shape (shape_of v) = 0’ >> fs []
+        >- rels_empty_tac >>
+        cases_on ‘size_of_shape (shape_of v) = 1’ >> fs []
+        >- (fs [shape_of_def, panLangTheory.size_of_shape_def] >> rels_empty_tac) >>
+        rels_empty_tac) >>
+       eval_call_nested_seq_impl_only_tac >>
+       strip_tac >> fs [] >>
+       ‘nctxt.eid_map = ctxt.eid_map’ by
+         fs [Abbr ‘nctxt’, ctxt_fc_eid_map_eq] >>
+       fs [] >>
+       cases_on ‘res1’ >> fs [] >> rveq >> fs [] >>
+       TRY (cases_on ‘x’ >> fs [] >> rveq >> fs []) >>
+       cases_on ‘FLOOKUP ctxt.eid_map eid’ >> fs [] >>
+       cases_on ‘x’ >> fs [] >>
+       rveq >> fs [] >>
+       cases_on ‘size_of_shape (shape_of v) = 0’ >> fs []
+       >- rels_empty_tac >>
+       cases_on ‘size_of_shape (shape_of v) = 1’ >> fs []
+       >- (
+        fs [shape_of_def, panLangTheory.size_of_shape_def] >>
+        rels_empty_tac) >>
+       rels_empty_tac) >>
+      rename [‘eid ≠ m'’] >>  (* a hack *)
       TOP_CASE_TAC >> fs []
       >- (
        eval_call_impl_only_tac >>
        strip_tac >> fs [] >>
-       cases_on ‘FLOOKUP ctxt.eid_map m'’ >> fs []
-       >- fs [Abbr ‘nctxt’, ctxt_fc_eid_map_eq] >>
        ‘nctxt.eid_map = ctxt.eid_map’ by
          fs [Abbr ‘nctxt’, ctxt_fc_eid_map_eq] >>
        fs [] >>
+       cases_on ‘FLOOKUP ctxt.eid_map eid’ >> fs [] >>
        cases_on ‘x’ >> fs [] >>
        cases_on ‘size_of_shape (shape_of v) = 0’ >> fs []
        >- rels_empty_tac >>
        cases_on ‘size_of_shape (shape_of v) = 1’ >> fs []
        >- (fs [shape_of_def, panLangTheory.size_of_shape_def] >> rels_empty_tac) >>
        rels_empty_tac) >>
-      (* I am here *)
-      eval_call_impl_only_tac >>
-      strip_tac >> fs [] >>
-      cases_on ‘FLOOKUP ctxt.eid_map m'’ >> fs []
-      >- fs [Abbr ‘nctxt’, ctxt_fc_eid_map_eq] >>
-      ‘nctxt.eid_map = ctxt.eid_map’ by
-        fs [Abbr ‘nctxt’, ctxt_fc_eid_map_eq] >>
-      fs [] >>
-      cases_on ‘x’ >> fs [] >>
-      ‘~MEM (uassigned_eid ctxt.eid_map) t.eids’ by (
-        fs [excp_rel_def] >> fs [uassigned_eid_def, shape_of_def, panLangTheory.size_of_shape_def]  >>
-        CCONTR_TAC >> fs [] >> fs [max_set_list_max, list_max_add_not_mem]) >>
-      cases_on ‘size_of_shape (shape_of v) = 0’ >> fs []
-      >- rels_empty_tac >>
-      cases_on ‘size_of_shape (shape_of v) = 1’ >> fs []
+      TOP_CASE_TAC >> fs [] >>
+      TOP_CASE_TAC >> fs []
       >- (
-       fs [shape_of_def, panLangTheory.size_of_shape_def] >>
-       rels_empty_tac) >>
-      rels_empty_tac) >>
-     TOP_CASE_TAC >> fs []
-     >- (
-      eval_call_impl_only_tac >>
-      strip_tac >> fs [] >>
-      cases_on ‘FLOOKUP ctxt.eid_map m'’ >> fs []
-      >- fs [Abbr ‘nctxt’, ctxt_fc_eid_map_eq] >>
-      ‘nctxt.eid_map = ctxt.eid_map’ by
-        fs [Abbr ‘nctxt’, ctxt_fc_eid_map_eq] >>
-      fs [] >>
-      cases_on ‘x’ >> fs [] >>
-      ‘~MEM (uassigned_eid ctxt.eid_map) t.eids’ by (
-        fs [excp_rel_def] >> fs [uassigned_eid_def, shape_of_def, panLangTheory.size_of_shape_def]  >>
-        CCONTR_TAC >> fs [] >> fs [max_set_list_max, list_max_add_not_mem]) >>
-      cases_on ‘size_of_shape (shape_of v) = 0’ >> fs []
-      >- rels_empty_tac >>
-      cases_on ‘size_of_shape (shape_of v) = 1’ >> fs []
-      >- (
-       fs [shape_of_def, panLangTheory.size_of_shape_def] >>
-       rels_empty_tac) >>
-      rels_empty_tac) >>
-     eval_call_nested_seq_impl_only_tac >>
-     strip_tac >> fs [] >>
-     ‘~MEM (uassigned_eid ctxt.eid_map) t.eids’ by (
-       fs [excp_rel_def] >> fs [uassigned_eid_def, shape_of_def, panLangTheory.size_of_shape_def]  >>
-       CCONTR_TAC >> fs [] >> fs [max_set_list_max, list_max_add_not_mem]) >>
-     cases_on ‘res1’ >> fs [] >> rveq >> fs [] >>
-     TRY (cases_on ‘x’ >> fs [] >> rveq >> fs []) >>
-     cases_on ‘FLOOKUP ctxt.eid_map m'’ >> fs []
-     >- fs [Abbr ‘nctxt’, ctxt_fc_eid_map_eq] >>
-     ‘nctxt.eid_map = ctxt.eid_map’ by
-       fs [Abbr ‘nctxt’, ctxt_fc_eid_map_eq] >>
-     fs [] >>
-     cases_on ‘x’ >> fs [] >>
-     cases_on ‘size_of_shape (shape_of v) = 0’ >> fs []
-     >- rels_empty_tac >>
-     cases_on ‘size_of_shape (shape_of v) = 1’ >> fs []
-     >- (
-      fs [shape_of_def, panLangTheory.size_of_shape_def] >>
-      rels_empty_tac) >>
-     rels_empty_tac)
-
-
-
-
-      ‘~MEM (uassigned_eid ctxt.eid_map) t.eids’ by (
-        fs [excp_rel_def] >> fs [uassigned_eid_def, shape_of_def, panLangTheory.size_of_shape_def]  >>
-        CCONTR_TAC >> fs [] >> fs [max_set_list_max, list_max_add_not_mem]) >>
-
-
-
-
-
-
-      cases_on ‘size_of_shape (shape_of v) = 0’ >> fs []
-      >- rels_empty_tac >>
+       TOP_CASE_TAC >> fs [] >>
+       eval_call_impl_only_tac >>
+       strip_tac >> fs [] >>
+       ‘nctxt.eid_map = ctxt.eid_map’ by
+         fs [Abbr ‘nctxt’, ctxt_fc_eid_map_eq] >>
+       fs [] >>
+       cases_on ‘FLOOKUP ctxt.eid_map eid’ >> fs [] >>
+       cases_on ‘x’ >> fs [] >>
+       cases_on ‘size_of_shape (shape_of v) = 0’ >> fs []
+       >- rels_empty_tac >>
        cases_on ‘size_of_shape (shape_of v) = 1’ >> fs []
        >- (fs [shape_of_def, panLangTheory.size_of_shape_def] >> rels_empty_tac) >>
-       rels_empty_tac)
-
-
-      )
-
-
-
-
-      )
-
-      )
-
-     >- (
-      cases_on ‘FLOOKUP ctxt.eid_map m'’ >> fs []
+       rels_empty_tac) >>
+      TOP_CASE_TAC >> fs [] >> rveq >> fs []
       >- (
+       eval_call_impl_only_tac >>
+       strip_tac >> fs [] >>
+       ‘nctxt.eid_map = ctxt.eid_map’ by
+         fs [Abbr ‘nctxt’, ctxt_fc_eid_map_eq] >>
+       fs [] >>
+       cases_on ‘FLOOKUP ctxt.eid_map eid’ >> fs [] >>
+       cases_on ‘x’ >> fs [] >>
+       cases_on ‘size_of_shape (shape_of v) = 0’ >> fs []
+       >- rels_empty_tac >>
+       cases_on ‘size_of_shape (shape_of v) = 1’ >> fs []
+       >- (fs [shape_of_def, panLangTheory.size_of_shape_def] >> rels_empty_tac) >>
+       rels_empty_tac) >>
+      eval_call_nested_seq_impl_only_tac >>
+      strip_tac >> fs [] >>
+      ‘nctxt.eid_map = ctxt.eid_map’ by
+        fs [Abbr ‘nctxt’, ctxt_fc_eid_map_eq] >>
+      fs [] >>
+      cases_on ‘res1’ >> fs [] >> rveq >> fs [] >>
+      TRY (cases_on ‘x’ >> fs [] >> rveq >> fs []) >>
+      cases_on ‘FLOOKUP ctxt.eid_map eid’ >> fs [] >>
+      cases_on ‘x’ >> fs [] >>
+      rveq >> fs [] >>
+      cases_on ‘size_of_shape (shape_of v) = 0’ >> fs []
+      >- rels_empty_tac >>
+      cases_on ‘size_of_shape (shape_of v) = 1’ >> fs []
+      >- (
+       fs [shape_of_def, panLangTheory.size_of_shape_def] >>
+       rels_empty_tac) >>
+      rels_empty_tac
+
+val handle_eid_one_evar_size_zero =
+      cases_on ‘is_valid_value s.locals evar v’ >> fs []
+      >- (
+       fs [is_valid_value_def] >>
+       cases_on ‘FLOOKUP s.locals evar’ >> fs [] >>
+       ‘~(shape_of x = One) /\ size_of_shape (shape_of x) = 0’ by (
+         drule locals_rel_lookup_ctxt >>
+         disch_then drule >> strip_tac >> fs [] >>
+         fs [length_flatten_eq_size_of_shape] >>
+         rveq >> cases_on ‘x’ >> TRY (cases_on ‘w’) >>
+         fs [shape_of_def, panLangTheory.size_of_shape_def]) >>
+       fs [] >> rveq >> fs [] >>
+       cases_on ‘m' = eid’ >> fs [] >> rveq >> fs []
+       >- (
+        TOP_CASE_TAC >> fs []
+        >- (
+         eval_call_impl_only_tac >>
+         strip_tac >> fs [] >>
+         ‘nctxt.eid_map = ctxt.eid_map’ by
+           fs [Abbr ‘nctxt’, ctxt_fc_eid_map_eq] >>
+         fs [] >>
+         cases_on ‘FLOOKUP ctxt.eid_map eid’ >> fs [] >>
+         cases_on ‘x'’ >> fs []
+         >- rels_empty_tac) >>
+        TOP_CASE_TAC >> fs [] >>
+        TOP_CASE_TAC >> fs []
+        >- (
+         TOP_CASE_TAC >> fs [] >> (
+         eval_call_impl_only_tac >>
+         strip_tac >> fs [] >>
+         ‘nctxt.eid_map = ctxt.eid_map’ by
+           fs [Abbr ‘nctxt’, ctxt_fc_eid_map_eq] >>
+         fs [] >>
+         cases_on ‘FLOOKUP ctxt.eid_map eid’ >> fs [] >>
+         cases_on ‘x'’ >> fs []
+         >- rels_empty_tac)) >>
+        TOP_CASE_TAC >> fs []
+        >- (
+         eval_call_impl_only_tac >>
+         strip_tac >> fs [] >>
+         ‘nctxt.eid_map = ctxt.eid_map’ by
+           fs [Abbr ‘nctxt’, ctxt_fc_eid_map_eq] >>
+         fs [] >>
+         cases_on ‘FLOOKUP ctxt.eid_map eid’ >> fs [] >>
+         cases_on ‘x'’ >> fs []
+         >- rels_empty_tac) >>
+        fs [nested_seq_def] >>
+        fs [evaluate_def] >> pairarg_tac >> fs [] >>
+        cases_on ‘eval t x0’ >> fs [] >>
+        cases_on ‘x'’ >> fs [] >>
+        ‘OPT_MMAP (eval t)
+         (FLAT (MAP FST (MAP (compile_exp ctxt) argexps))) = SOME (FLAT (MAP flatten args))’ by (
+          fs [opt_mmap_eq_some] >> metis_tac [eval_map_comp_exp_flat_eq]) >>
+        fs [] >>
+        fs [panSemTheory.lookup_code_def, CaseEq "option", CaseEq "prod"] >> rveq >>
+        drule code_rel_imp >>
+        disch_then drule >>
+        strip_tac >> fs [] >>
+        fs [lookup_code_def] >>
+        drule (INST_TYPE [``:'c``|->``:num``] list_rel_length_shape_of_flatten) >>
+        disch_then (qspec_then ‘ns’ mp_tac) >>
+        fs [] >>
+        cases_on ‘ t.clock = 0’ >- fs [state_rel_def] >>
+        fs [] >> rveq >>
+        qmatch_asmsub_abbrev_tac ‘compile_prog nctxt _,nt’ >>
+        first_x_assum (qspecl_then [‘nt’, ‘nctxt’] mp_tac) >>
+        impl_tac
+        >- (
+         fs [Abbr ‘nctxt’, Abbr ‘nt’, slc_tlc_rw] >>
+         match_mp_tac call_preserve_state_code_locals_rel >>
+         fs []) >>
+        strip_tac >> fs [] >>
+        ‘nctxt.eid_map = ctxt.eid_map’ by
+          fs [Abbr ‘nctxt’, ctxt_fc_eid_map_eq] >>
+        fs [] >>
+        cases_on ‘res1’ >> fs [] >> rveq >> fs [] >>
+        TRY (cases_on ‘x’ >> fs [] >> rveq >> fs []) >>
+        cases_on ‘FLOOKUP ctxt.eid_map eid’ >> fs [] >>
+        cases_on ‘x’ >> fs [] >>
+        rveq >> fs [] >>
+        rels_empty_tac) >>
+       (* m' <> eid *)
+       rename [‘eid ≠ m'’] >>
+       TOP_CASE_TAC >> fs []
+       >- (
+        eval_call_impl_only_tac >>
+        strip_tac >> fs [] >>
+        ‘nctxt.eid_map = ctxt.eid_map’ by
+          fs [Abbr ‘nctxt’, ctxt_fc_eid_map_eq] >>
+        fs [] >>
+        cases_on ‘FLOOKUP ctxt.eid_map eid’ >> fs [] >>
+        cases_on ‘x'’ >> fs [] >>
+        cases_on ‘size_of_shape (shape_of v) = 0’ >> fs []
+        >- rels_empty_tac >>
+        cases_on ‘size_of_shape (shape_of v) = 1’ >> fs []
+        >- (fs [shape_of_def, panLangTheory.size_of_shape_def] >> rels_empty_tac) >>
+        rels_empty_tac) >>
+       TOP_CASE_TAC >> fs [] >>
+       TOP_CASE_TAC >> fs []
+       >- (
+        TOP_CASE_TAC >> fs []
+        >- (
+         eval_call_impl_only_tac >>
+         strip_tac >> fs [] >>
+         ‘nctxt.eid_map = ctxt.eid_map’ by
+           fs [Abbr ‘nctxt’, ctxt_fc_eid_map_eq] >>
+         fs [] >>
+         cases_on ‘FLOOKUP ctxt.eid_map eid’ >> fs [] >>
+         cases_on ‘x'’ >> fs [] >>
+         cases_on ‘size_of_shape (shape_of v) = 0’ >> fs []
+         >- rels_empty_tac >>
+         cases_on ‘size_of_shape (shape_of v) = 1’ >> fs []
+         >- (fs [shape_of_def, panLangTheory.size_of_shape_def] >> rels_empty_tac) >>
+         rels_empty_tac) >>
+        eval_call_impl_only_tac >>
+        strip_tac >> fs [] >>
+        ‘nctxt.eid_map = ctxt.eid_map’ by
+          fs [Abbr ‘nctxt’, ctxt_fc_eid_map_eq] >>
+        fs [] >>
+        cases_on ‘FLOOKUP ctxt.eid_map eid’ >> fs [] >>
+        cases_on ‘x'’ >> fs [] >>
+        cases_on ‘size_of_shape (shape_of v) = 0’ >> fs []
+        >- rels_empty_tac >>
+        cases_on ‘size_of_shape (shape_of v) = 1’ >> fs []
+        >- (fs [shape_of_def, panLangTheory.size_of_shape_def] >> rels_empty_tac) >>
+        rels_empty_tac) >>
+       TOP_CASE_TAC >> fs [] >> rveq >> fs []
+       >- (
+        eval_call_impl_only_tac >>
+        strip_tac >> fs [] >>
+        ‘nctxt.eid_map = ctxt.eid_map’ by
+          fs [Abbr ‘nctxt’, ctxt_fc_eid_map_eq] >>
+        fs [] >>
+        cases_on ‘FLOOKUP ctxt.eid_map eid’ >> fs [] >>
+        cases_on ‘x'’ >> fs [] >>
+        cases_on ‘size_of_shape (shape_of v) = 0’ >> fs []
+        >- rels_empty_tac >>
+        cases_on ‘size_of_shape (shape_of v) = 1’ >> fs []
+        >- (fs [shape_of_def, panLangTheory.size_of_shape_def] >> rels_empty_tac) >>
+        rels_empty_tac) >>
+       fs [nested_seq_def] >>
+       fs [evaluate_def] >> pairarg_tac >> fs [] >>
+       cases_on ‘eval t x0’ >> fs [] >>
+       cases_on ‘x'’ >> fs [] >>
+       ‘OPT_MMAP (eval t)
+        (FLAT (MAP FST (MAP (compile_exp ctxt) argexps))) = SOME (FLAT (MAP flatten args))’ by (
+          fs [opt_mmap_eq_some] >> metis_tac [eval_map_comp_exp_flat_eq]) >>
+       fs [] >>
        fs [panSemTheory.lookup_code_def, CaseEq "option", CaseEq "prod"] >> rveq >>
        drule code_rel_imp >>
        disch_then drule >>
@@ -5997,594 +6022,745 @@ Proof
        drule (INST_TYPE [``:'c``|->``:num``] list_rel_length_shape_of_flatten) >>
        disch_then (qspec_then ‘ns’ mp_tac) >>
        fs [] >>
-       strip_tac >>
-       qmatch_asmsub_abbrev_tac ‘compile_prog nctxt _’ >>
-       first_x_assum (qspecl_then
-                      [‘dec_clock t with
-                        locals := FEMPTY |++ ZIP (ns,FLAT (MAP flatten args))’,
-                       ‘nctxt’] mp_tac) >>
+       cases_on ‘ t.clock = 0’ >- fs [state_rel_def] >>
+       fs [] >> rveq >>
+       qmatch_asmsub_abbrev_tac ‘compile_prog nctxt _,nt’ >>
+       first_x_assum (qspecl_then [‘nt’, ‘nctxt’] mp_tac) >>
        impl_tac
        >- (
-        fs [Abbr ‘nctxt’, slc_tlc_rw] >>
+        fs [Abbr ‘nctxt’, Abbr ‘nt’, slc_tlc_rw] >>
         match_mp_tac call_preserve_state_code_locals_rel >>
         fs []) >>
        strip_tac >> fs [] >>
-       rfs [Abbr ‘nctxt’, ctxt_fc_eid_map_eq]) >>
-
-
-      )
-     >- call_tail_ret_impl_tac >>
-
-
-
-     TOP_CASE_TAC >> fs [] >>
-
-    call_tail_ret_impl_tac >>
-    cases_on ‘FLOOKUP ctxt.eid_map m'’ >> fs [] >>
-   cases_on ‘x’ >> fs []
-
-    cases_on ‘FLOOKUP s.locals rt’ >> fs [] >>
-
-
-
-    TOP_CASE_TAC >> fs [] >>
-    TOP_CASE_TAC >> fs []
-    >- (
-     TOP_CASE_TAC >> fs []
-     >- (
-      fs [locals_rel_def] >> first_x_assum drule >> fs [] >>
-      fs [OPT_MMAP_def] >>
-      strip_tac >> fs [] >>
-      pop_assum (assume_tac o GSYM) >>
-      ‘size_of_shape (shape_of x) = 1’ by
-        fs [panLangTheory.size_of_shape_def, shape_of_def] >>
-      fs [GSYM length_flatten_eq_size_of_shape] >> rfs [flatten_def]) >>
-
-
-
-                           )
-
-
-
-     dec_clock t with
-           locals := FEMPTY |++ ZIP (ns,FLAT (MAP flatten args))
-
-           FLOOKUP ctxt.code_vars fname = SOME (vshapes,ns)
- ctxt_fc ctxt.code_vars ctxt.eid_map (MAP FST vshapes)
-             (MAP SND vshapes) ns
-
-     TOP_CASE_TAC >> fs []
-       )
-
-
-
-
-
-
-    )
-    cheat
-QED
-
-
-
-
-
-
-
-
-      )
-      )
-
-
-
-
-
-
-     )
-
-
-
-      )
-       )
-
-
-
-
-
-    )
-
-
-   >- (
-    cases_on ‘m' = eid’ >> fs [] >>
-    >- (
-     cases_on ‘FLOOKUP s.eshapes eid’
-     >- (
-      ‘FLOOKUP ctxt.eid_map eid = NONE’ by cheat >> fs [] >>
-      rveq >>
-      TOP_CASE_TAC >> fs []
-      >- cheat >>
-      cheat) >>
-     rveq >>
-     ‘FLOOKUP ctxt.eid_map eid <> NONE’ by cheat >> fs [] >>
-     TOP_CASE_TAC >> fs [] >>
-     TOP_CASE_TAC >> fs [] >>
-     TOP_CASE_TAC >> fs []
-     >- (
+       ‘nctxt.eid_map = ctxt.eid_map’ by
+         fs [Abbr ‘nctxt’, ctxt_fc_eid_map_eq] >>
+       fs [] >>
+       cases_on ‘res1’ >> fs [] >> rveq >> fs [] >>
+       TRY (cases_on ‘x'’ >> fs [] >> rveq >> fs []) >>
+       cases_on ‘FLOOKUP ctxt.eid_map eid’ >> fs [] >>
+       cases_on ‘x'’ >> fs [] >>
+       rveq >> fs [] >>
+       cases_on ‘size_of_shape (shape_of v) = 0’ >> fs []
+       >- rels_empty_tac >>
+       cases_on ‘size_of_shape (shape_of v) = 1’ >> fs []
+       >- (
+        fs [shape_of_def, panLangTheory.size_of_shape_def] >>
+        rels_empty_tac) >>
+       rels_empty_tac) >>
+      cases_on ‘m' = eid’ >> fs [] >> rveq >> fs []
+      >- (
+       TOP_CASE_TAC >> fs []
+       >- (
+        eval_call_impl_only_tac >>
+        strip_tac >> fs [] >>
+        ‘nctxt.eid_map = ctxt.eid_map’ by
+          fs [Abbr ‘nctxt’, ctxt_fc_eid_map_eq] >>
+          fs [] >> rveq >> fs [] >>
+          cases_on ‘FLOOKUP ctxt.eid_map eid’ >> fs [] >>
+          cases_on ‘x’ >> fs [] >>
+          cases_on ‘size_of_shape (shape_of v) = 0’ >> fs []
+          >- rels_empty_tac >>
+          cases_on ‘size_of_shape (shape_of v) = 1’ >> fs []
+          >- (
+           fs [shape_of_def, panLangTheory.size_of_shape_def] >>
+           rels_empty_tac) >>
+          rels_empty_tac) >>
+         TOP_CASE_TAC >> fs [] >>
+         TOP_CASE_TAC >> fs []
+         >- (
+          TOP_CASE_TAC >> fs [] >>
+          eval_call_impl_only_tac >>
+          strip_tac >> fs [] >>
+          ‘nctxt.eid_map = ctxt.eid_map’ by
+            fs [Abbr ‘nctxt’, ctxt_fc_eid_map_eq] >>
+          fs [] >>
+          cases_on ‘FLOOKUP ctxt.eid_map eid’ >> fs [] >>
+          cases_on ‘x’ >> fs [] >> rveq >> fs [] >>
+          cases_on ‘size_of_shape (shape_of v) = 0’ >> fs []
+          >- rels_empty_tac >>
+          cases_on ‘size_of_shape (shape_of v) = 1’ >> fs []
+          >- (
+           fs [shape_of_def, panLangTheory.size_of_shape_def] >>
+           rels_empty_tac) >>
+          rels_empty_tac) >>
+         TOP_CASE_TAC >> fs []
+         >- (
+          eval_call_impl_only_tac >>
+          strip_tac >> fs [] >>
+          ‘nctxt.eid_map = ctxt.eid_map’ by
+            fs [Abbr ‘nctxt’, ctxt_fc_eid_map_eq] >>
+          fs [] >> rveq >> fs [] >>
+          cases_on ‘FLOOKUP ctxt.eid_map eid’ >> fs [] >>
+          cases_on ‘x’ >> fs [] >>
+          cases_on ‘size_of_shape (shape_of v) = 0’ >> fs []
+          >- rels_empty_tac >>
+          cases_on ‘size_of_shape (shape_of v) = 1’ >> fs []
+          >- (
+           fs [shape_of_def, panLangTheory.size_of_shape_def] >>
+           rels_empty_tac) >>
+          rels_empty_tac) >>
+         fs [nested_seq_def] >>
+         fs [evaluate_def] >> pairarg_tac >> fs [] >>
+         cases_on ‘eval t x0’ >> fs [] >>
+         cases_on ‘x’ >> fs [] >>
+         ‘OPT_MMAP (eval t)
+          (FLAT (MAP FST (MAP (compile_exp ctxt) argexps))) = SOME (FLAT (MAP flatten args))’ by (
+           fs [opt_mmap_eq_some] >> metis_tac [eval_map_comp_exp_flat_eq]) >>
+         fs [] >>
+         fs [panSemTheory.lookup_code_def, CaseEq "option", CaseEq "prod"] >> rveq >>
+         drule code_rel_imp >>
+         disch_then drule >>
+         strip_tac >> fs [] >>
+         fs [lookup_code_def] >>
+         drule (INST_TYPE [``:'c``|->``:num``] list_rel_length_shape_of_flatten) >>
+         disch_then (qspec_then ‘ns’ mp_tac) >>
+         fs [] >>
+         cases_on ‘ t.clock = 0’ >- fs [state_rel_def] >>
+         fs [] >> rveq >>
+         qmatch_asmsub_abbrev_tac ‘compile_prog nctxt _,nt’ >>
+         first_x_assum (qspecl_then [‘nt’, ‘nctxt’] mp_tac) >>
+         impl_tac
+         >- (
+          fs [Abbr ‘nctxt’, Abbr ‘nt’, slc_tlc_rw] >>
+          match_mp_tac call_preserve_state_code_locals_rel >>
+          fs []) >>
+         strip_tac >> fs [] >>
+         ‘nctxt.eid_map = ctxt.eid_map’ by
+           fs [Abbr ‘nctxt’, ctxt_fc_eid_map_eq] >>
+         fs [] >>
+         cases_on ‘res1’ >> fs [] >> rveq >> fs [] >>
+         TRY (cases_on ‘x’ >> fs [] >> rveq >> fs []) >>
+         cases_on ‘FLOOKUP ctxt.eid_map eid’ >> fs [] >>
+         cases_on ‘x’ >> fs [] >>
+        rveq >> fs [] >>
+        rels_empty_tac) >>
       TOP_CASE_TAC >> fs []
       >- (
-       fs [is_valid_value_def] >>
-       cases_on ‘FLOOKUP s.locals m’ >> fs []
-       >- ( cheat ) >>
-       cheat (* from local_rel *) ) >>
+       eval_call_impl_only_tac >>
+       strip_tac >> fs [] >>
+       ‘nctxt.eid_map = ctxt.eid_map’ by
+         fs [Abbr ‘nctxt’, ctxt_fc_eid_map_eq] >>
+       fs [] >>
+       cases_on ‘FLOOKUP ctxt.eid_map m'’ >> fs [] >>
+       cases_on ‘x’ >> fs [] >>
+       cases_on ‘size_of_shape (shape_of v) = 0’ >> fs []
+       >- rels_empty_tac >>
+       cases_on ‘size_of_shape (shape_of v) = 1’ >> fs []
+       >- (
+        fs [shape_of_def, panLangTheory.size_of_shape_def] >>
+        rels_empty_tac) >>
+       rels_empty_tac) >>
       TOP_CASE_TAC >> fs [] >>
       TOP_CASE_TAC >> fs []
       >- (
-       fs [is_valid_value_def] >>
-       cases_on ‘FLOOKUP s.locals m’ >> fs []
+       TOP_CASE_TAC >> fs []
        >- (
-        >> rveq >> fs [] >> cheat) >>
-       cheat) >>
-      cheat) >>
-
-
-
-
-
-
-
-
-
-
-  rename [‘FLOOKUP ctxt.eid_map eid’] >>
-  TOP_CASE_TAC >> fs []
-  >- (
-   rename [‘FLOOKUP ctxt.var_nums rt’] >>
-   TOP_CASE_TAC >> fs []
-   >- (
-    cases_on ‘evaluate (prog,dec_clock s with locals := newlocals)’ >> fs [] >>
-    eval_handler_impl_only_tac >>
-    strip_tac >> fs [] >>
-    cases_on ‘v3’ >> fs [] >> rveq >> fs []
-    >- rels_empty_tac
-    >- (
-     cases_on ‘is_valid_value s.locals rt v’ >> fs [] >>
-     fs [is_valid_value_def] >> cases_on ‘FLOOKUP s.locals rt’ >> fs [] >>
-     fs [locals_rel_def] >> last_x_assum drule_all >> fs [])
-    >- (
-     cases_on ‘FLOOKUP nctxt.eid_map m'’ >> fs [] >>
-     cases_on ‘x’ >> fs [] >>
-     cases_on ‘m' = eid’ >> fs [] >> rveq
-     >- fs [Abbr ‘nctxt’, ctxt_fc_eid_map_eq] >>
-     cases_on ‘size_of_shape (shape_of v) = 0’ >> fs []
-     >- rels_empty_tac >>
-     cases_on ‘size_of_shape (shape_of v) = 1’ >> fs []
-     >- (
-      fs [shape_of_def, panLangTheory.size_of_shape_def] >>
-      rels_empty_tac) >>
-     rels_empty_tac) >>
-    rels_empty_tac) >>
-   cases_on ‘evaluate (prog,dec_clock s with locals := newlocals)’ >> fs [] >>
-   cases_on ‘q’ >> fs [] >> cases_on ‘x'’ >> fs [] >> rveq >> fs []
-   >- (
-    TOP_CASE_TAC >> fs [] >>
-    TOP_CASE_TAC >> fs []
-    >- (
-     TOP_CASE_TAC >> fs [] >>
-     call_tail_ret_impl_tac) >>
-    TOP_CASE_TAC >> fs []
-    >- call_tail_ret_impl_tac >>
-    call_nested_seq_ret_impl_tac)
-   >- (
-    cases_on ‘is_valid_value s.locals rt v’ >> fs [] >>
-    TOP_CASE_TAC >> fs [] >>
-    TOP_CASE_TAC >> fs []
-    >- (
-     TOP_CASE_TAC >> fs []
-     >- (
-      fs [is_valid_value_def] >>
-      cases_on ‘FLOOKUP s.locals rt’ >> fs [] >>
-      drule locals_rel_lookup_ctxt >>
-      disch_then drule >> strip_tac >>
-      fs [length_flatten_eq_size_of_shape] >>
-      rfs [panLangTheory.size_of_shape_def]) >>
-     eval_call_impl_only_tac >>
-     strip_tac >> fs [] >>
-     fs [is_valid_value_def] >>
-     cases_on ‘FLOOKUP s.locals rt’ >> fs [] >>
-     ‘size_of_shape (shape_of v) = 1’ by (
-       fs [locals_rel_def] >>
-       last_x_assum drule >>
-       fs [shape_of_def]) >>
-     fs [state_rel_def, panSemTheory.set_var_def,set_var_def,
-         Abbr ‘nctxt’, code_rel_def, ctxt_fc_code_vars_eq,ctxt_fc_eid_map_eq,
-         panSemTheory.set_var_def,set_var_def] >>
-     conj_tac
-     >- (
-      fs [excp_rel_def, ctxt_fc_code_vars_eq,ctxt_fc_eid_map_eq,
-          panSemTheory.set_var_def,set_var_def] >> rw [] >>
-      res_tac >> fs []) >>
-     ‘size_of_shape (shape_of v) = 1’ by fs [] >>
-      drule locals_rel_lookup_ctxt >>
-      disch_then drule >> strip_tac >> fs [] >>
-      rveq >> fs [length_flatten_eq_size_of_shape] >>
-      rfs [panLangTheory.size_of_shape_def] >>
-      fs [locals_rel_def, panSemTheory.set_var_def,set_var_def] >>
-      rw [] >> rveq >>
-      fs [FLOOKUP_UPDATE] >>
-      FULL_CASE_TAC >> fs [] >> rveq >>
-      rfs [shape_of_def, panLangTheory.size_of_shape_def]
+        eval_call_impl_only_tac >>
+        strip_tac >> fs [] >>
+        ‘nctxt.eid_map = ctxt.eid_map’ by
+          fs [Abbr ‘nctxt’, ctxt_fc_eid_map_eq] >>
+        fs [] >>
+        cases_on ‘FLOOKUP ctxt.eid_map m'’ >> fs [] >>
+        cases_on ‘x’ >> fs [] >>
+        cases_on ‘size_of_shape (shape_of v) = 0’ >> fs []
+        >- rels_empty_tac >>
+        cases_on ‘size_of_shape (shape_of v) = 1’ >> fs []
+        >- (
+         fs [shape_of_def, panLangTheory.size_of_shape_def] >>
+         rels_empty_tac) >>
+        rels_empty_tac) >>
+       eval_call_impl_only_tac >>
+       strip_tac >> fs [] >>
+       ‘nctxt.eid_map = ctxt.eid_map’ by
+         fs [Abbr ‘nctxt’, ctxt_fc_eid_map_eq] >>
+       fs [] >>
+       cases_on ‘FLOOKUP ctxt.eid_map m'’ >> fs [] >>
+       cases_on ‘x’ >> fs [] >>
+       cases_on ‘size_of_shape (shape_of v) = 0’ >> fs []
+       >- rels_empty_tac >>
+       cases_on ‘size_of_shape (shape_of v) = 1’ >> fs []
+       >- (
+        fs [shape_of_def, panLangTheory.size_of_shape_def] >>
+        rels_empty_tac) >>
+       rels_empty_tac) >>
+      TOP_CASE_TAC >> fs []
       >- (
-       fs [OPT_MMAP_def, FLOOKUP_UPDATE] >> rveq >>
-       fs [length_flatten_eq_size_of_shape, panLangTheory.size_of_shape_def]) >>
-      res_tac >> fs [] >>
-      match_mp_tac opt_mmap_flookup_update >>
+       eval_call_impl_only_tac >>
+       strip_tac >> fs [] >>
+       ‘nctxt.eid_map = ctxt.eid_map’ by
+         fs [Abbr ‘nctxt’, ctxt_fc_eid_map_eq] >>
+       fs [] >>
+       cases_on ‘FLOOKUP ctxt.eid_map m'’ >> fs [] >>
+       cases_on ‘x’ >> fs [] >>
+       cases_on ‘size_of_shape (shape_of v) = 0’ >> fs []
+       >- rels_empty_tac >>
+       cases_on ‘size_of_shape (shape_of v) = 1’ >> fs []
+       >- (
+        fs [shape_of_def, panLangTheory.size_of_shape_def] >>
+        rels_empty_tac) >>
+       rels_empty_tac) >>
+      fs [nested_seq_def] >>
+      fs [evaluate_def] >> pairarg_tac >> fs [] >>
+      cases_on ‘eval t x0’ >> fs [] >>
+      cases_on ‘x’ >> fs [] >>
+      ‘OPT_MMAP (eval t)
+       (FLAT (MAP FST (MAP (compile_exp ctxt) argexps))) = SOME (FLAT (MAP flatten args))’ by (
+        fs [opt_mmap_eq_some] >> metis_tac [eval_map_comp_exp_flat_eq]) >>
       fs [] >>
-      drule no_overlap_flookup_distinct >>
-      disch_then drule_all >> fs [distinct_lists_def]) >>
-    fs [is_valid_value_def] >>
-    cases_on ‘FLOOKUP s.locals rt’ >> fs [] >>
-    TOP_CASE_TAC >> fs []
-    >- (
-     ‘LENGTH r' = 1’ by (
-       drule_all locals_rel_lookup_ctxt >> strip_tac >>
-       fs [length_flatten_eq_size_of_shape] >>
-       rfs [panLangTheory.size_of_shape_def]) >>
-     fs [] >> eval_call_impl_only_tac >>
-     strip_tac >> fs [] >>
-     ‘size_of_shape (shape_of x) = 1’ by (
-       drule_all locals_rel_lookup_ctxt >> strip_tac >>
-       fs [locals_rel_def] >>
-       last_x_assum drule >>
-       fs [shape_of_def, length_flatten_eq_size_of_shape,
-           panLangTheory.size_of_shape_def]) >>
-     fs [state_rel_def, panSemTheory.set_var_def,set_var_def,
-         Abbr ‘nctxt’, code_rel_def, ctxt_fc_code_vars_eq,ctxt_fc_eid_map_eq,
-         panSemTheory.set_var_def,set_var_def] >>
-     conj_tac
-     >- (
-      fs [excp_rel_def, ctxt_fc_code_vars_eq,ctxt_fc_eid_map_eq,
-          panSemTheory.set_var_def,set_var_def] >> rw [] >>
-      res_tac >> fs []) >>
-     ‘size_of_shape (shape_of v) = 1’ by fs [] >>
-     drule locals_rel_lookup_ctxt >>
-     disch_then drule >> strip_tac >> fs [] >>
-     rveq >> fs [length_flatten_eq_size_of_shape] >>
-     rfs [panLangTheory.size_of_shape_def] >>
-     fs [locals_rel_def, panSemTheory.set_var_def,set_var_def] >>
-     rw [] >> rveq >>
-     fs [FLOOKUP_UPDATE] >>
-     FULL_CASE_TAC >> fs [] >> rveq >>
-     rfs [shape_of_def, panLangTheory.size_of_shape_def]
-     >- (
-      cases_on ‘ns'’ >> fs [] >>
-      fs [OPT_MMAP_def, FLOOKUP_UPDATE, ooHD_def] >> rveq >>
-      fs [length_flatten_eq_size_of_shape, panLangTheory.size_of_shape_def, shape_of_def]) >>
-     res_tac >> fs [] >>
-     match_mp_tac opt_mmap_flookup_update >>
-     fs [] >> cases_on ‘ns'’ >> fs [ooHD_def] >> rveq >>
-     imp_res_tac no_overlap_flookup_distinct >>
-     fs [distinct_lists_def]) >>
-    fs [nested_seq_def] >>
-    fs [evaluate_def] >> pairarg_tac >> fs [] >>
-    cases_on ‘eval t x0’ >> fs [] >>
-    cases_on ‘x'’ >> fs [] >>
-    ‘OPT_MMAP (eval t)
-     (FLAT (MAP FST (MAP (compile_exp ctxt) argexps))) = SOME (FLAT (MAP flatten args))’ by (
-      fs [opt_mmap_eq_some] >> metis_tac [eval_map_comp_exp_flat_eq]) >>
-    fs [] >>
-    fs [panSemTheory.lookup_code_def, CaseEq "option", CaseEq "prod"] >> rveq >>
-    drule code_rel_imp >>
-    disch_then drule >>
-    strip_tac >> fs [] >>
-    fs [lookup_code_def] >>
-    drule (INST_TYPE [``:'c``|->``:num``] list_rel_length_shape_of_flatten) >>
-    disch_then (qspec_then ‘ns’ mp_tac) >>
-    fs [] >>
-    cases_on ‘ t.clock = 0’ >- fs [state_rel_def] >>
-    fs [] >> rveq >>
-    qmatch_asmsub_abbrev_tac ‘compile_prog nctxt _,nt’ >>
-    first_x_assum (qspecl_then [‘nt’, ‘nctxt’] mp_tac) >>
-    impl_tac
-    >- (
-     fs [Abbr ‘nctxt’, Abbr ‘nt’, slc_tlc_rw] >>
-     match_mp_tac call_preserve_state_code_locals_rel >>
-     fs []) >>
-    strip_tac >> fs [] >>
-    cases_on ‘res1’ >> fs [] >>
-    cases_on ‘x'’ >> fs [] >>
-    cases_on ‘size_of_shape (shape_of x) = 0’ >> fs []
-    >- (
-     rveq >> drule locals_rel_lookup_ctxt >>
-     disch_then (qspecl_then [‘rt’, ‘x’] assume_tac) >>
-     fs [length_flatten_eq_size_of_shape] >> rfs [] >> rveq >>
-     fs [set_var_def, panSemTheory.set_var_def] >>
-     fs [nested_seq_def, evaluate_def] >>
-     conj_tac >- fs [state_rel_def] >>
-     conj_tac >- fs [Abbr ‘nctxt’, code_rel_def, ctxt_fc_code_vars_eq, ctxt_fc_eid_map_eq] >>
-     conj_tac
-     >- (
-      fs [Abbr ‘nctxt’, excp_rel_def, ctxt_fc_code_vars_eq, ctxt_fc_eid_map_eq] >>
-      rw [] >> last_x_assum drule_all >> fs []) >>
-     fs [locals_rel_def] >> rw [] >>
-     fs [FLOOKUP_UPDATE] >> FULL_CASE_TAC >> fs [] >> rveq
-     >- (
-      fs [OPT_MMAP_def] >>
-      ‘LENGTH (flatten v) = 0’ suffices_by fs[] >>
-      rewrite_tac [length_flatten_eq_size_of_shape] >>
-      fs []) >>
-     first_x_assum drule >> strip_tac >> fs [] >>
-     fs [opt_mmap_eq_some, MAP_EQ_EVERY2, LIST_REL_EL_EQN] >>
-     rw [] >> fs [FLOOKUP_UPDATE] >>
-     TOP_CASE_TAC >> fs [] >>
-     drule ctxt_max_el_leq >>
-     qpat_x_assum ‘LENGTH _ = LENGTH (flatten _)’ (assume_tac o GSYM) >>
-     fs [] >> disch_then drule_all >> fs []) >>
-    ‘1 < size_of_shape (shape_of x)’ by (
-      drule locals_rel_lookup_ctxt >>
+      fs [panSemTheory.lookup_code_def, CaseEq "option", CaseEq "prod"] >> rveq >>
+      drule code_rel_imp >>
       disch_then drule >>
-      strip_tac >> fs [] >> rfs [] >>
-      fs [panLangTheory.size_of_shape_def] >>
-      DECIDE_TAC) >>
-    fs [] >>
-    ‘ALL_DISTINCT r'’ by
-      (fs [locals_rel_def] >> imp_res_tac all_distinct_flookup_all_distinct) >>
-    fs [globals_lookup_def] >>
-    drule evaluate_seq_assign_load_globals >>
-    disch_then (qspecl_then [‘t1 with locals :=
-                              t.locals |+ (ctxt.max_var + 1,Word 0w)’, ‘0w’] mp_tac) >>
-    impl_tac
-    >- (
-     conj_tac
-     >- (
-      fs [word_0_n2w] >>
-      imp_res_tac locals_rel_lookup_ctxt >> rveq >>
-      fs [length_flatten_eq_size_of_shape] >> rfs []) >>
-     conj_tac
-     >- (
-      rw [] >>
-      ‘n <> ctxt.max_var + 1’ suffices_by (
-         fs [FLOOKUP_UPDATE, locals_rel_def] >>
-         first_x_assum drule_all >> strip_tac >> fs [] >> rveq >>
-         imp_res_tac opt_mmap_mem_func >> fs []) >>
-      fs [locals_rel_def, ctxt_max_def] >>
-      last_x_assum drule_all >> strip_tac >> fs []) >>
-     rw [] >> rfs [] >>
-     drule locals_rel_lookup_ctxt >>
-     ‘size_of_shape (shape_of x) = LENGTH r'’ by (
-       drule locals_rel_lookup_ctxt >>
-       disch_then drule >>
-       strip_tac >> fs [] >> rveq >>
-       fs [length_flatten_eq_size_of_shape] >> rfs []) >>
-     fs [] >> drule opt_mmap_mem_func >>
-     disch_then drule >> strip_tac >> fs []) >>
-    strip_tac >> rveq >>
-    fs [set_var_def, panSemTheory.set_var_def,
-        panLangTheory.size_of_shape_def, shape_of_def] >>
-    conj_tac >- fs [state_rel_def] >>
-    conj_tac >- fs [Abbr ‘nctxt’, code_rel_def, ctxt_fc_code_vars_eq, ctxt_fc_eid_map_eq] >>
-    conj_tac
-    >- (
-     fs [Abbr ‘nctxt’, excp_rel_def, ctxt_fc_code_vars_eq, ctxt_fc_eid_map_eq] >>
-     rw [] >>last_x_assum drule_all >> fs []) >>
-    ‘MAP (λn. THE (FLOOKUP t1.globals n)) (GENLIST (λx. n2w x) (LENGTH r')) =
-     flatten v’ by (
-      fs [opt_mmap_eq_some] >>
-      ‘size_of_shape (shape_of v) = LENGTH r'’ by (
-        drule locals_rel_lookup_ctxt >>
-        disch_then drule >>
-        strip_tac >> fs [] >> rveq >>
-        fs [length_flatten_eq_size_of_shape] >> rfs []) >>
-      fs [] >> drule map_some_the_map >> fs []) >>
-    fs [] >>
-    match_mp_tac local_rel_le_zip_update_preserved >> fs [] >>
-    match_mp_tac local_rel_gt_max_var_preserved >>
-    fs [])
-   >- (
-    cases_on ‘m' = eid’ >> fs [] >> rveq >> rfs []
-    >- (
-     reverse (cases_on ‘FLOOKUP s.eshapes eid’) >> fs []
-     >- (fs [excp_rel_def] >> res_tac >> fs []) >>
-     rveq >> TOP_CASE_TAC >> fs [] >>
-     fs [panSemTheory.lookup_code_def, CaseEq "option", CaseEq "prod"] >> rveq >>
-     drule code_rel_imp >>
-     disch_then drule >>
-     strip_tac >> fs [] >>
-     fs [lookup_code_def] >>
-     drule (INST_TYPE [``:'c``|->``:num``] list_rel_length_shape_of_flatten) >>
-     disch_then (qspec_then ‘ns’ mp_tac) >>
-     fs [] >>
-     strip_tac >>
-     qmatch_asmsub_abbrev_tac ‘compile_prog nctxt _’ >>
-     first_x_assum (qspecl_then
-                    [‘dec_clock t with
-                      locals := FEMPTY |++ ZIP (ns,FLAT (MAP flatten args))’,
-                     ‘nctxt’] mp_tac) >>
-     impl_tac
-     >- (
-      fs [Abbr ‘nctxt’, slc_tlc_rw] >>
-      match_mp_tac call_preserve_state_code_locals_rel >>
-      fs []) >>
-     strip_tac >> fs [] >>
-     rfs [Abbr ‘nctxt’, ctxt_fc_eid_map_eq]) >>
-
-    TOP_CASE_TAC >> fs [] >>
-    TOP_CASE_TAC >> fs [] >>
-
-    call_tail_ret_impl_tac >>
-    cases_on ‘FLOOKUP ctxt.eid_map m'’ >> fs [] >>
-   cases_on ‘x’ >> fs []
-
-    cases_on ‘FLOOKUP s.locals rt’ >> fs [] >>
-
-
-
-    TOP_CASE_TAC >> fs [] >>
-    TOP_CASE_TAC >> fs []
-    >- (
-     TOP_CASE_TAC >> fs []
-     >- (
-      fs [locals_rel_def] >> first_x_assum drule >> fs [] >>
-      fs [OPT_MMAP_def] >>
       strip_tac >> fs [] >>
-      pop_assum (assume_tac o GSYM) >>
-      ‘size_of_shape (shape_of x) = 1’ by
-        fs [panLangTheory.size_of_shape_def, shape_of_def] >>
-      fs [GSYM length_flatten_eq_size_of_shape] >> rfs [flatten_def]) >>
+      fs [lookup_code_def] >>
+      drule (INST_TYPE [``:'c``|->``:num``] list_rel_length_shape_of_flatten) >>
+      disch_then (qspec_then ‘ns’ mp_tac) >>
+      fs [] >>
+      cases_on ‘ t.clock = 0’ >- fs [state_rel_def] >>
+      fs [] >> rveq >>
+      qmatch_asmsub_abbrev_tac ‘compile_prog nctxt _,nt’ >>
+      first_x_assum (qspecl_then [‘nt’, ‘nctxt’] mp_tac) >>
+      impl_tac
+      >- (
+       fs [Abbr ‘nctxt’, Abbr ‘nt’, slc_tlc_rw] >>
+       match_mp_tac call_preserve_state_code_locals_rel >>
+       fs []) >>
+      strip_tac >> fs [] >>
+      ‘nctxt.eid_map = ctxt.eid_map’ by
+        fs [Abbr ‘nctxt’, ctxt_fc_eid_map_eq] >>
+      fs [] >>
+      cases_on ‘res1’ >> fs [] >> rveq >> fs [] >>
+      TRY (cases_on ‘x’ >> fs [] >> rveq >> fs []) >>
+      cases_on ‘FLOOKUP ctxt.eid_map m'’ >> fs [] >>
+      cases_on ‘x’ >> fs [] >>
+      rveq >> fs [] >>
+      rels_empty_tac
 
 
 
-                           )
+val eval_call_impl_only'_tac =
+         fs [evaluate_def] >>
+         TOP_CASE_TAC >> fs [] >>
+         TOP_CASE_TAC >> fs [] >>
+         ‘OPT_MMAP (eval t)
+          (FLAT (MAP FST (MAP (compile_exp ctxt) argexps))) = SOME (FLAT (MAP flatten args))’ by (
+           fs [opt_mmap_eq_some] >> metis_tac [eval_map_comp_exp_flat_eq]) >>
+         fs [] >>
+         fs [panSemTheory.lookup_code_def, CaseEq "option", CaseEq "prod"] >> rveq >>
+         drule code_rel_imp >>
+         disch_then drule >>
+         strip_tac >> fs [] >>
+         fs [lookup_code_def] >>
+         drule (INST_TYPE [``:'c``|->``:num``] list_rel_length_shape_of_flatten) >>
+         disch_then (qspec_then ‘ns’ mp_tac) >>
+         fs [] >>
+         strip_tac >>
+         TOP_CASE_TAC >- fs [state_rel_def] >>
+         qmatch_goalsub_abbrev_tac ‘compile_prog nctxt _,nt’ >>
+         last_x_assum (qspecl_then [‘nt’, ‘nctxt’] mp_tac) >>
+         impl_tac
+         >- (
+          fs [Abbr ‘nctxt’, Abbr ‘nt’, slc_tlc_rw] >>
+          match_mp_tac call_preserve_state_code_locals_rel >>
+          fs [])
+
+val lookup_evar_one_ret_case =
+         first_x_assum drule >>
+         strip_tac >> rfs [] >>
+         eval_call_impl_only'_tac >>
+         strip_tac >> fs [] >>
+         ‘nctxt.eid_map = ctxt.eid_map’ by
+           fs [Abbr ‘nctxt’, ctxt_fc_eid_map_eq] >>
+         fs [] >>
+         cases_on ‘FLOOKUP ctxt.eid_map eid’ >> fs [] >>
+         cases_on ‘x'’ >> fs [] >> rveq >> fs [] >>
+         first_x_assum (qspecl_then [‘set_var h (HD (flatten v)) (t1 with locals := t.locals)’, ‘ctxt’] mp_tac) >>
+         impl_tac
+         >- (
+          fs [Abbr ‘nctxt’, Abbr ‘nt’, state_rel_def, set_var_def, panSemTheory.set_var_def] >>
+          conj_tac
+          >- (
+           fs [code_rel_def] >> rw [] >> res_tac >> fs [ctxt_fc_code_vars_eq]) >>
+          conj_tac
+          >- (
+           fs[excp_rel_def] >> rw [] >> res_tac >> fs [ctxt_fc_eid_map_eq]) >>
+          drule locals_rel_lookup_ctxt >>
+          disch_then drule >> strip_tac >> fs [] >>
+          fs [length_flatten_eq_size_of_shape] >>
+          rfs [] >> cases_on ‘t'’ >> fs [shape_of_def, panLangTheory.size_of_shape_def] >>
+          fs [locals_rel_def] >>
+          rw [] >> fs [FLOOKUP_UPDATE] >>
+          FULL_CASE_TAC >> fs [] >> rveq
+          >- (
+           fs [OPT_MMAP_def] >>
+           fs [FLOOKUP_UPDATE] >>
+           rfs [length_flatten_eq_size_of_shape,
+                panLangTheory.size_of_shape_def]) >>
+          first_x_assum drule >> strip_tac >> fs [] >>
+          ‘~ MEM h ns''’ by (
+            fs [no_overlap_def] >>
+            res_tac >> fs [] >> metis_tac []) >>
+          fs [opt_mmap_eq_some] >>
+          fs [MAP_EQ_EVERY2, LIST_REL_EL_EQN] >>
+          rw [] >> fs [FLOOKUP_UPDATE] >>
+          TOP_CASE_TAC >> fs []  >>
+          metis_tac [EL_MEM]) >>
+         strip_tac >> fs [] >>
+         ‘MEM r' t.eids’ suffices_by fs [] >>
+         fs [excp_rel_def] >>
+         ‘r' ∈ (IMAGE SND (FRANGE ctxt.eid_map))’
+         suffices_by metis_tac [set_eq_membership] >>
+         fs [IN_IMAGE, FRANGE_FLOOKUP] >>
+         qexists_tac ‘(One, r')’ >> fs [] >>
+         qexists_tac ‘eid’ >> fs []
+
+
+val lookup_evar_one_nested_ret_case =
+         qpat_x_assum ‘SOME (Label fname) = eval t x0’ (assume_tac o GSYM) >>
+         qmatch_goalsub_abbrev_tac ‘evaluate (Seq (AppCode x0 ar) pc, _)’ >>
+         drule evaluate_append_code_intro >>
+         fs [panSemTheory.lookup_code_def, CaseEq "option", CaseEq "prod"] >> rveq >>
+         drule code_rel_imp >>
+         disch_then drule >>
+         strip_tac >> fs [] >>
+         fs [lookup_code_def] >>
+         drule (INST_TYPE [``:'c``|->``:num``] list_rel_length_shape_of_flatten) >>
+         disch_then (qspec_then ‘ns’ mp_tac) >>
+         fs [] >> strip_tac >>
+         disch_then (qspecl_then [‘pc’, ‘ar’] assume_tac) >>
+         fs [] >> pop_assum kall_tac >>
+         qmatch_goalsub_abbrev_tac ‘evaluate (pc, tnew)’ >>
+
+        first_x_assum drule >>
+        strip_tac >> rfs [] >>
+        fs [Abbr ‘pc’] >>
+        fs [evaluate_def] >>
+        ‘eval tnew x0 = eval t x0’ by cheat >>
+        fs [] >>
+        ‘OPT_MMAP (eval tnew)
+         (FLAT (MAP FST (MAP (compile_exp ctxt) argexps))) = SOME (FLAT (MAP flatten args))’ by (
+          (*fs [opt_mmap_eq_some] >> metis_tac [eval_map_comp_exp_flat_eq]*) cheat) >>
+        fs [Abbr ‘tnew’, lookup_code_def] >>
+        drule (INST_TYPE [``:'c``|->``:num``] list_rel_length_shape_of_flatten) >>
+        disch_then (qspec_then ‘ns’ mp_tac) >>
+        fs [FLOOKUP_UPDATE] >>
+        cases_on ‘ t.clock = 0’ >- fs [state_rel_def] >>
+        fs [] >> rveq >>
+        fs [evaluate_def] >> pairarg_tac >> fs [] >>
+        qmatch_asmsub_abbrev_tac ‘compile_prog nctxt _,nt’ >>
+        last_x_assum (qspecl_then [‘nt’, ‘nctxt’] mp_tac) >>
+        impl_tac
+        >- ( cheat
+         (*fs [Abbr ‘nctxt’, Abbr ‘nt’, slc_tlc_rw] >>
+         match_mp_tac call_preserve_state_code_locals_rel >>
+         fs [] *)) >>
+        strip_tac >> fs [] >>
+        ‘nctxt.eid_map = ctxt.eid_map’ by
+          fs [Abbr ‘nctxt’, ctxt_fc_eid_map_eq] >>
+        fs [] >>
+         cases_on ‘FLOOKUP ctxt.eid_map eid’ >> fs [] >>
+         cases_on ‘x'’ >> fs [] >> rveq >> fs [] >>
+         ‘MEM r' t.eids’ by (
+           fs [excp_rel_def] >>
+           ‘r' ∈ (IMAGE SND (FRANGE ctxt.eid_map))’
+           suffices_by metis_tac [set_eq_membership] >>
+           fs [IN_IMAGE, FRANGE_FLOOKUP] >>
+           qexists_tac ‘(One, r')’ >> fs [] >>
+           qexists_tac ‘eid’ >> fs []) >>
+         fs [] >>
+         first_x_assum (qspecl_then [‘set_var h (HD (flatten v)) (s1' with locals := t.locals)’, ‘ctxt’] mp_tac) >>
+         impl_tac
+         >- (
+          fs [Abbr ‘nctxt’, Abbr ‘nt’, state_rel_def, set_var_def, panSemTheory.set_var_def] >>
+          conj_tac
+          >- (
+           fs [code_rel_def] >> rw [] >> res_tac >> fs [ctxt_fc_code_vars_eq]) >>
+          conj_tac
+          >- (
+           fs[excp_rel_def] >> rw [] >> res_tac >> fs [ctxt_fc_eid_map_eq]) >>
+          drule locals_rel_lookup_ctxt >>
+          disch_then drule >> strip_tac >> fs [] >>
+          fs [length_flatten_eq_size_of_shape] >>
+          rfs [] >> cases_on ‘t'’ >> fs [shape_of_def, panLangTheory.size_of_shape_def] >>
+          fs [locals_rel_def] >>
+          rw [] >> fs [FLOOKUP_UPDATE] >>
+          FULL_CASE_TAC >> fs [] >> rveq
+          >- (
+           fs [OPT_MMAP_def] >>
+           fs [FLOOKUP_UPDATE] >>
+           rfs [length_flatten_eq_size_of_shape,
+                panLangTheory.size_of_shape_def]) >>
+          first_x_assum drule >> strip_tac >> fs [] >>
+          ‘~ MEM h ns''’ by (
+            fs [no_overlap_def] >>
+            res_tac >> fs [] >> metis_tac []) >>
+          fs [opt_mmap_eq_some] >>
+          fs [MAP_EQ_EVERY2, LIST_REL_EL_EQN] >>
+          rw [] >> fs [FLOOKUP_UPDATE] >>
+          TOP_CASE_TAC >> fs []  >>
+          metis_tac [EL_MEM]) >>
+         strip_tac >> fs [] >> rveq >> fs []
+
+val call_rest_diff_eids_impl_tac =
+       eval_call_impl_only_tac >>
+       strip_tac >> fs [] >>
+       ‘nctxt.eid_map = ctxt.eid_map’ by
+         fs [Abbr ‘nctxt’, ctxt_fc_eid_map_eq] >>
+       fs [] >>
+       cases_on ‘FLOOKUP ctxt.eid_map eid’ >> fs [] >>
+       cases_on ‘x'’ >> fs [] >>
+       cases_on ‘size_of_shape (shape_of v) = 0’ >> fs [] >>
+       ‘r'' <> r'’ by (
+         fs [excp_rel_def] >>
+         first_x_assum drule >>
+         disch_then (qspecl_then [‘m'’, ‘One’] mp_tac) >> fs []) >> fs []
+       >- (rels_empty_tac >> strip_tac >> fs [panLangTheory.size_of_shape_def]) >>
+       cases_on ‘size_of_shape (shape_of v) = 1’ >> fs []
+       >- (fs [shape_of_def, panLangTheory.size_of_shape_def] >> rels_empty_tac) >>
+       fs [panLangTheory.size_of_shape_def] >>
+       rels_empty_tac
+
+
+val call_rest_diff_eids_nested_impl_tac =
+      qpat_x_assum ‘SOME (Label fname) = eval t x0’ (assume_tac o GSYM) >>
+      qmatch_goalsub_abbrev_tac ‘evaluate (Seq (AppCode x0 ar) pc, _)’ >>
+      drule eval_upde_code_eq >>
+      fs [panSemTheory.lookup_code_def, CaseEq "option", CaseEq "prod"] >> rveq >>
+      drule code_rel_imp >>
+      disch_then drule >>
+      strip_tac >> fs [] >>
+      fs [lookup_code_def] >>
+      drule (INST_TYPE [``:'c``|->``:num``] list_rel_length_shape_of_flatten) >>
+      disch_then (qspec_then ‘ns’ mp_tac) >>
+      fs [] >> strip_tac >>
+      disch_then (qspecl_then [‘pc’, ‘ar’] assume_tac) >>
+      fs [] >> pop_assum kall_tac >>
+      qmatch_goalsub_abbrev_tac ‘evaluate (pc, tnew)’ >>
+      fs [Abbr ‘pc’] >>
+      fs [evaluate_def] >>
+      ‘eval tnew x0 = eval t x0’ by cheat >>
+      fs [] >>
+      ‘OPT_MMAP (eval tnew)
+       (FLAT (MAP FST (MAP (compile_exp ctxt) argexps))) = SOME (FLAT (MAP flatten args))’ by (
+        (*fs [opt_mmap_eq_some] >> metis_tac [eval_map_comp_exp_flat_eq]*) cheat) >>
+      fs [Abbr ‘tnew’, lookup_code_def] >>
+      drule (INST_TYPE [``:'c``|->``:num``] list_rel_length_shape_of_flatten) >>
+      disch_then (qspec_then ‘ns’ mp_tac) >>
+      fs [FLOOKUP_UPDATE] >>
+      cases_on ‘ t.clock = 0’ >- fs [state_rel_def] >>
+      fs [] >> rveq >>
+      fs [evaluate_def] >> pairarg_tac >> fs [] >>
+      qmatch_asmsub_abbrev_tac ‘compile_prog nctxt _,nt’ >>
+      last_x_assum (qspecl_then [‘nt’, ‘nctxt’] mp_tac) >>
+      impl_tac
+      >- ( cheat
+         (*fs [Abbr ‘nctxt’, Abbr ‘nt’, slc_tlc_rw] >>
+           match_mp_tac call_preserve_state_code_locals_rel >>
+           fs [] *)) >>
+      strip_tac >> fs [] >>
+      ‘nctxt.eid_map = ctxt.eid_map’ by
+        fs [Abbr ‘nctxt’, ctxt_fc_eid_map_eq] >>
+      fs [] >> rveq >> fs [] >>
+      cases_on ‘FLOOKUP ctxt.eid_map eid’ >> fs [] >>
+      cases_on ‘x'’ >> fs [] >> rveq >> fs [] >>
+      ‘r''' <> r'’ by (
+        fs [excp_rel_def] >>
+        first_x_assum drule >>
+        disch_then (qspecl_then [‘m'’, ‘One’] mp_tac) >> fs []) >>
+      fs [] >>
+      fs [shape_of_def, panLangTheory.size_of_shape_def] >> rels_empty_tac
 
 
 
-     dec_clock t with
-           locals := FEMPTY |++ ZIP (ns,FLAT (MAP flatten args))
 
-           FLOOKUP ctxt.code_vars fname = SOME (vshapes,ns)
- ctxt_fc ctxt.code_vars ctxt.eid_map (MAP FST vshapes)
-             (MAP SND vshapes) ns
-
-     TOP_CASE_TAC >> fs []
-      )
-
-
-       )
-
-
-     )
-
-
-
-    )
-
-
-
-
-
-
-
-
-
-
-
-
-
-
-
-
-
-
-    rveq >> fs [] >>
-    fs [Abbr ‘nctxt’, state_rel_def, ctxt_fc_code_vars_eq, ctxt_fc_eid_map_eq,
-        empty_locals_def, panSemTheory.empty_locals_def, code_rel_def, ctxt_fc_eid_map_eq, excp_rel_def] >>
-    rw [] >> first_x_assum drule_all >> fs []
-    >- (
-     cases_on ‘res1’ >> fs [] >>
-     cases_on ‘x’ >> fs [] >>
-     fs [set_var_def] >> rveq >>
+val is_valid_evar_one_case_tac =
+      fs [is_valid_value_def] >>
+      cases_on ‘FLOOKUP s.locals evar’ >> fs [] >>
+      ‘shape_of x = One /\ size_of_shape (shape_of x) = 1’ by (
+        drule locals_rel_lookup_ctxt >>
+        disch_then drule >> strip_tac >> fs [] >>
+        fs [length_flatten_eq_size_of_shape] >>
+        rveq >> cases_on ‘x’ >> TRY (cases_on ‘w’) >>
+        fs [shape_of_def, panLangTheory.size_of_shape_def]) >>
+      fs [] >> rveq >> fs [] >>
+      cases_on ‘m' = eid’ >> fs [] >> rveq >> fs []
+      >- (
+       TOP_CASE_TAC >> fs []
+       >- lookup_evar_one_ret_case >>
+       TOP_CASE_TAC >> fs [] >>
+       TOP_CASE_TAC >> fs []
+       >- (
+        TOP_CASE_TAC >> fs []
+        >- lookup_evar_one_ret_case >>
+        lookup_evar_one_ret_case) >>
+       TOP_CASE_TAC >> fs []
+       >- lookup_evar_one_ret_case >>
+       lookup_evar_one_nested_ret_case) >>
+      rename [‘eid ≠ m'’] >>
+      TOP_CASE_TAC >> fs []
+      >- call_rest_diff_eids_impl_tac >>
+      TOP_CASE_TAC >> fs [] >>
+      TOP_CASE_TAC >> fs []
+      >- (
+       TOP_CASE_TAC >> fs []
+       >- call_rest_diff_eids_impl_tac >>
+       call_rest_diff_eids_impl_tac) >>
+      TOP_CASE_TAC >> fs []
+      >- (
+       rename [‘Handle (ooHD sm) _ _’] >>
+       call_rest_diff_eids_impl_tac) >>
+      call_rest_diff_eids_nested_impl_tac
 
 
-
-
-     )
-
-
-
-
-
-
-
-    call_nested_seq_ret_impl_tac
-
-
-
-
-
-      )
-
-     )
-
-    )
-
-     call_tail_ret_impl_tac
-
-
-     )
+Theorem compile_Call:
+  ^(get_goal "compile_prog _ (panLang$Call _ _ _)")
+Proof
+   abc_tac >>
+   (* Handler case *)
+   rename [‘FLOOKUP ctxt.eid_map eid’] >>
+   cases_on ‘evaluate (prog,dec_clock s with locals := newlocals)’ >>
+   fs [] >> cases_on ‘q’ >> fs [] >> cases_on ‘x’ >> fs []
+   >- time_out_handle_tac
+   >- return_handle_tac
+   >- ((* Exception case *)
+    rename [‘FLOOKUP ctxt.var_nums rt’] >>
     TOP_CASE_TAC >> fs []
-    >- call_tail_ret_impl_tac >>
-    call_tail_ret_impl_tac)
-
-
-
-     )
-
-    )
-
-
-
-
-
-
-
-
-   TOP_CASE_TAC >> fs [] >>
-   TOP_CASE_TAC >> fs [] >>
-   TOP_CASE_TAC >> fs []
-   >- (
-    cases_on ‘evaluate (prog,dec_clock s with locals := newlocals)’ >> fs [] >>
-    cases_on ‘q’ >> fs [] >> cases_on ‘x’ >> fs [] >> rveq >> fs []
+    >-  excp_eid_none_handler_tac >>
+    (* eid = SOME case *)
+    cases_on ‘FLOOKUP s.eshapes eid’ >> fs []
     >- (
-     cases_on ‘evaluate (prog,dec_clock s with locals := newlocals)’ >> fs [] >>
-     call_tail_ret_impl_tac)
+     fs [excp_rel_def] >>
+     drule fdom_eq_flookup_none >>
+     disch_then drule >> fs []) >>
+    TOP_CASE_TAC >> fs [] >>
+    reverse TOP_CASE_TAC >> fs []
+    >- cheat (* eid = SOME Comb *) >>
+    (* eid = SOME One *)
+    ‘x' = One’ by (fs [excp_rel_def] >> res_tac >> fs []) >>
+    fs [] >>
+    rename [‘FLOOKUP ctxt.var_nums evar’] >>
+    TOP_CASE_TAC >> fs []
+    (* evar = NONE case *)
+    >- handle_eid_one_evar_none >>
+    (* evar = SOME case *)
+    TOP_CASE_TAC >> fs [] >>
+    TOP_CASE_TAC >> fs []
+    (* lookup evar = (q, []) *)
+    >- handle_eid_one_evar_size_zero >>
+    TOP_CASE_TAC
     >- (
-     cases_on ‘is_valid_value s.locals rt v’ >> fs [] >>
-     fs [is_valid_value_def] >> cases_on ‘FLOOKUP s.locals rt’ >> fs [] >>
-     drule_all locals_rel_lookup_ctxt >> strip_tac >> fs [] >>
-     fs  [length_flatten_eq_size_of_shape] >>
-     rfs [panLangTheory.size_of_shape_def, shape_of_def])
-    >- (
-     cases_on ‘m' = eid’ >> fs [] >> rveq
-     >- (
-      reverse (cases_on ‘FLOOKUP s.eshapes eid’) >> fs [] >> rveq
-      >- (fs [excp_rel_def] >> last_x_assum drule_all >> fs []) >>
-      fs [] >> cheat  (* tricky *)) >>
-     eval_call_impl_only_tac >>
-     strip_tac >> fs [] >>
-     cases_on ‘FLOOKUP nctxt.eid_map m'’ >> fs [] >>
-     cases_on ‘x’ >> fs [] >>
-     cases_on ‘size_of_shape (shape_of v) = 0’ >> fs []
-     >- rels_empty_tac >>
-     cases_on ‘size_of_shape (shape_of v) = 1’ >> fs []
-     >- (fs [shape_of_def, panLangTheory.size_of_shape_def] >> rels_empty_tac) >>
-     rels_empty_tac) >>
-    call_tail_ret_impl_tac)
-   >- (
-    cases_on ‘evaluate (prog,dec_clock s with locals := newlocals)’ >> fs [] >>
-    cases_on ‘q’ >> fs [] >> cases_on ‘x’ >> fs [] >> rveq >> fs []
-    >- call_tail_ret_impl_tac
-    >- (
-     cases_on ‘evaluate (prog,dec_clock s with locals := newlocals)’ >> fs [] >>
-     eval_call_impl_only_tac
-     strip_tac >> fs [] >>
-     cases_on ‘is_valid_value s.locals rt v’ >> fs [] >>
-     ‘size_of_shape (shape_of v) = 1’ by cheat >> fs [] >> rveq >>
-     fs [GSYM length_flatten_eq_size_of_shape] >> cases_on ‘flatten v’ >> fs [] >>
-     rveq >> fs [] >>
-     fs [state_rel_def, Abbr ‘nctxt’, code_rel_def, ctxt_fc_code_vars_eq, set_var_def,
-         panSemTheory.set_var_def, panSemTheory.empty_locals_def,
-         empty_locals_def, ctxt_fc_eid_map_eq] >>
-     conj_tac
-     >- (
-      fs [excp_rel_def, ctxt_fc_eid_map_eq] >> rw [] >>
-      res_tac >> fs []) >>
-     fs [locals_rel_def] >> rw [] >>
-     fs [FLOOKUP_UPDATE] >>
-     cases_on ‘vname = rt’ >> fs [] >> rveq
-     >- cheat >>
-     cheat) >> cheat) >> cheat) >> cheat
+     (* lookup evar = (One, h::t') *)
+     cases_on ‘is_valid_value s.locals evar v’ >> fs []
+     >- is_valid_evar_one_case_tac  >>
+
+
+
+
+     cases_on ‘m' = eid’ >> fs [] >> rveq >> fs []
+      >- (
+       TOP_CASE_TAC >> fs []
+       >- (
+        eval_call_impl_only_tac >>
+        strip_tac >> fs [] >>
+        ‘nctxt.eid_map = ctxt.eid_map’ by
+          fs [Abbr ‘nctxt’, ctxt_fc_eid_map_eq] >>
+          fs [] >> rveq >> fs [] >>
+          cases_on ‘FLOOKUP ctxt.eid_map eid’ >> fs [] >>
+          cases_on ‘x’ >> fs [] >> rveq >> fs []
+
+
+
+          cases_on ‘size_of_shape (shape_of v) = 0’ >> fs []
+          >- rels_empty_tac >>
+          cases_on ‘size_of_shape (shape_of v) = 1’ >> fs []
+          >- (
+           fs [shape_of_def, panLangTheory.size_of_shape_def] >>
+           rels_empty_tac) >>
+          rels_empty_tac) >>
+         TOP_CASE_TAC >> fs [] >>
+         TOP_CASE_TAC >> fs []
+         >- (
+          TOP_CASE_TAC >> fs [] >>
+          eval_call_impl_only_tac >>
+          strip_tac >> fs [] >>
+          ‘nctxt.eid_map = ctxt.eid_map’ by
+            fs [Abbr ‘nctxt’, ctxt_fc_eid_map_eq] >>
+          fs [] >>
+          cases_on ‘FLOOKUP ctxt.eid_map eid’ >> fs [] >>
+          cases_on ‘x’ >> fs [] >> rveq >> fs [] >>
+          cases_on ‘size_of_shape (shape_of v) = 0’ >> fs []
+          >- rels_empty_tac >>
+          cases_on ‘size_of_shape (shape_of v) = 1’ >> fs []
+          >- (
+           fs [shape_of_def, panLangTheory.size_of_shape_def] >>
+           rels_empty_tac) >>
+          rels_empty_tac) >>
+         TOP_CASE_TAC >> fs []
+         >- (
+          eval_call_impl_only_tac >>
+          strip_tac >> fs [] >>
+          ‘nctxt.eid_map = ctxt.eid_map’ by
+            fs [Abbr ‘nctxt’, ctxt_fc_eid_map_eq] >>
+          fs [] >> rveq >> fs [] >>
+          cases_on ‘FLOOKUP ctxt.eid_map eid’ >> fs [] >>
+          cases_on ‘x’ >> fs [] >>
+          cases_on ‘size_of_shape (shape_of v) = 0’ >> fs []
+          >- rels_empty_tac >>
+          cases_on ‘size_of_shape (shape_of v) = 1’ >> fs []
+          >- (
+           fs [shape_of_def, panLangTheory.size_of_shape_def] >>
+           rels_empty_tac) >>
+          rels_empty_tac) >>
+         fs [nested_seq_def] >>
+         fs [evaluate_def] >> pairarg_tac >> fs [] >>
+         cases_on ‘eval t x0’ >> fs [] >>
+         cases_on ‘x’ >> fs [] >>
+         ‘OPT_MMAP (eval t)
+          (FLAT (MAP FST (MAP (compile_exp ctxt) argexps))) = SOME (FLAT (MAP flatten args))’ by (
+           fs [opt_mmap_eq_some] >> metis_tac [eval_map_comp_exp_flat_eq]) >>
+         fs [] >>
+         fs [panSemTheory.lookup_code_def, CaseEq "option", CaseEq "prod"] >> rveq >>
+         drule code_rel_imp >>
+         disch_then drule >>
+         strip_tac >> fs [] >>
+         fs [lookup_code_def] >>
+         drule (INST_TYPE [``:'c``|->``:num``] list_rel_length_shape_of_flatten) >>
+         disch_then (qspec_then ‘ns’ mp_tac) >>
+         fs [] >>
+         cases_on ‘ t.clock = 0’ >- fs [state_rel_def] >>
+         fs [] >> rveq >>
+         qmatch_asmsub_abbrev_tac ‘compile_prog nctxt _,nt’ >>
+         first_x_assum (qspecl_then [‘nt’, ‘nctxt’] mp_tac) >>
+         impl_tac
+         >- (
+          fs [Abbr ‘nctxt’, Abbr ‘nt’, slc_tlc_rw] >>
+          match_mp_tac call_preserve_state_code_locals_rel >>
+          fs []) >>
+         strip_tac >> fs [] >>
+         ‘nctxt.eid_map = ctxt.eid_map’ by
+           fs [Abbr ‘nctxt’, ctxt_fc_eid_map_eq] >>
+         fs [] >>
+         cases_on ‘res1’ >> fs [] >> rveq >> fs [] >>
+         TRY (cases_on ‘x’ >> fs [] >> rveq >> fs []) >>
+         cases_on ‘FLOOKUP ctxt.eid_map eid’ >> fs [] >>
+         cases_on ‘x’ >> fs [] >>
+        rveq >> fs [] >>
+        rels_empty_tac) >>
+      TOP_CASE_TAC >> fs []
+      >- (
+       eval_call_impl_only_tac >>
+       strip_tac >> fs [] >>
+       ‘nctxt.eid_map = ctxt.eid_map’ by
+         fs [Abbr ‘nctxt’, ctxt_fc_eid_map_eq] >>
+       fs [] >>
+       cases_on ‘FLOOKUP ctxt.eid_map m'’ >> fs [] >>
+       cases_on ‘x’ >> fs [] >>
+       cases_on ‘size_of_shape (shape_of v) = 0’ >> fs []
+       >- rels_empty_tac >>
+       cases_on ‘size_of_shape (shape_of v) = 1’ >> fs []
+       >- (
+        fs [shape_of_def, panLangTheory.size_of_shape_def] >>
+        rels_empty_tac) >>
+       rels_empty_tac) >>
+      TOP_CASE_TAC >> fs [] >>
+      TOP_CASE_TAC >> fs []
+      >- (
+       TOP_CASE_TAC >> fs []
+       >- (
+        eval_call_impl_only_tac >>
+        strip_tac >> fs [] >>
+        ‘nctxt.eid_map = ctxt.eid_map’ by
+          fs [Abbr ‘nctxt’, ctxt_fc_eid_map_eq] >>
+        fs [] >>
+        cases_on ‘FLOOKUP ctxt.eid_map m'’ >> fs [] >>
+        cases_on ‘x’ >> fs [] >>
+        cases_on ‘size_of_shape (shape_of v) = 0’ >> fs []
+        >- rels_empty_tac >>
+        cases_on ‘size_of_shape (shape_of v) = 1’ >> fs []
+        >- (
+         fs [shape_of_def, panLangTheory.size_of_shape_def] >>
+         rels_empty_tac) >>
+        rels_empty_tac) >>
+       eval_call_impl_only_tac >>
+       strip_tac >> fs [] >>
+       ‘nctxt.eid_map = ctxt.eid_map’ by
+         fs [Abbr ‘nctxt’, ctxt_fc_eid_map_eq] >>
+       fs [] >>
+       cases_on ‘FLOOKUP ctxt.eid_map m'’ >> fs [] >>
+       cases_on ‘x’ >> fs [] >>
+       cases_on ‘size_of_shape (shape_of v) = 0’ >> fs []
+       >- rels_empty_tac >>
+       cases_on ‘size_of_shape (shape_of v) = 1’ >> fs []
+       >- (
+        fs [shape_of_def, panLangTheory.size_of_shape_def] >>
+        rels_empty_tac) >>
+       rels_empty_tac) >>
+      TOP_CASE_TAC >> fs []
+      >- (
+       eval_call_impl_only_tac >>
+       strip_tac >> fs [] >>
+       ‘nctxt.eid_map = ctxt.eid_map’ by
+         fs [Abbr ‘nctxt’, ctxt_fc_eid_map_eq] >>
+       fs [] >>
+       cases_on ‘FLOOKUP ctxt.eid_map m'’ >> fs [] >>
+       cases_on ‘x’ >> fs [] >>
+       cases_on ‘size_of_shape (shape_of v) = 0’ >> fs []
+       >- rels_empty_tac >>
+       cases_on ‘size_of_shape (shape_of v) = 1’ >> fs []
+       >- (
+        fs [shape_of_def, panLangTheory.size_of_shape_def] >>
+        rels_empty_tac) >>
+       rels_empty_tac) >>
+      fs [nested_seq_def] >>
+      fs [evaluate_def] >> pairarg_tac >> fs [] >>
+      cases_on ‘eval t x0’ >> fs [] >>
+      cases_on ‘x’ >> fs [] >>
+      ‘OPT_MMAP (eval t)
+       (FLAT (MAP FST (MAP (compile_exp ctxt) argexps))) = SOME (FLAT (MAP flatten args))’ by (
+        fs [opt_mmap_eq_some] >> metis_tac [eval_map_comp_exp_flat_eq]) >>
+      fs [] >>
+      fs [panSemTheory.lookup_code_def, CaseEq "option", CaseEq "prod"] >> rveq >>
+      drule code_rel_imp >>
+      disch_then drule >>
+      strip_tac >> fs [] >>
+      fs [lookup_code_def] >>
+      drule (INST_TYPE [``:'c``|->``:num``] list_rel_length_shape_of_flatten) >>
+      disch_then (qspec_then ‘ns’ mp_tac) >>
+      fs [] >>
+      cases_on ‘ t.clock = 0’ >- fs [state_rel_def] >>
+      fs [] >> rveq >>
+      qmatch_asmsub_abbrev_tac ‘compile_prog nctxt _,nt’ >>
+      first_x_assum (qspecl_then [‘nt’, ‘nctxt’] mp_tac) >>
+      impl_tac
+      >- (
+       fs [Abbr ‘nctxt’, Abbr ‘nt’, slc_tlc_rw] >>
+       match_mp_tac call_preserve_state_code_locals_rel >>
+       fs []) >>
+      strip_tac >> fs [] >>
+      ‘nctxt.eid_map = ctxt.eid_map’ by
+        fs [Abbr ‘nctxt’, ctxt_fc_eid_map_eq] >>
+      fs [] >>
+      cases_on ‘res1’ >> fs [] >> rveq >> fs [] >>
+      TRY (cases_on ‘x’ >> fs [] >> rveq >> fs []) >>
+      cases_on ‘FLOOKUP ctxt.eid_map m'’ >> fs [] >>
+      cases_on ‘x’ >> fs [] >>
+      rveq >> fs [] >>
+      rels_empty_tac
+
+
+
+
+
+
+
+
+
+     ) >>
+    cheat) >>
+   cheat
 QED
 
-QED
+
+
 
 
 val _ = export_theory();
